---
chapter: complex-numbers
topic: de-moivres-theorem
jee_frequency: 7
years_appeared: [2003, 2018, 2019, 2020, 2021, 2023, 2025]
question_count: 15
difficulty: medium
question_types: ['mcq', 'integer']
exams: ['mains']
---

# Complex Numbers: De Moivres Theorem

**JEE Frequency**: Appeared in **7 years** (2003 - 2025)

**Question Count**: 15 questions

## Question Types

- **MCQ**: 12 questions
- **INTEGER**: 3 questions

## Difficulty Distribution

- **Easy**: 4 questions
- **Medium**: 11 questions

## Worked Examples

### Example 1 (Year: 2003)

**Question:**

If $${\left( {{{1 + i} \over {1 - i}}} \right)^x} = 1$$ then :

**Solution:**

$${\left( {{{1 + i} \over {1 - i}}} \right)^x} = 1$$
<br><br>$$ \Rightarrow $$ $${\left[ {{{\left( {1 + i} \right)\left( {1 + i} \right)} \over {\left( {1 - i} \right)\left( {1 + i} \right)}}} \right]^x} = 1$$
<br><br>$$ \Rightarrow $$ $${\left[ {{{{{\left( {1 + i} \right)}^2}} \over {1 - {i^2}}}} \right]^x} = 1$$
<br><br>$$ \Rightarrow $$ $${\left[ {{{1 + 2i + {i^2}} \over {1 + 1}}} \right]^x} = 1$$
<br><br>$$ \Rightarrow $$ $${\left[ {{{1 + 2i - 1} \over 2}} \right]^x} = 1$$
<br><br>$$ \Rightarrow {\left( i \right)^x} = 1$$
<br><br>We know $$i = \sqrt { - 1} $$
<br><br>$$\therefore$$ $${i^2} =  - 1$$
<br><br>$$ \Rightarrow $$ $${i^3} =  - 1 \times i =  - i$$
<br><br>$$ \Rightarrow $$ $${i^4} =  - i \times i =  - {i^2} =  - \left( { - 1} \right) = 1$$
<br><br>So when power of $$i$$ is 4 or multiple of 4 then it's value is = 1
<br><br>$$\therefore$$ $${\left( i \right)^x} = 1$$ $$ = {\left( i \right)^{4n}}$$ where n is a positive integer.

### Example 2 (Year: 2018)

**Question:**

The least positive integer n for which $${\left( {{{1 + i\sqrt 3 } \over {1 - i\sqrt 3 }}} \right)^n} = 1,$$ is :

**Solution:**

$${\left( {{{1 + i\sqrt 3 } \over {1 - i\sqrt 3 }}} \right)^n} = 1$$
<br><br>$$ \Rightarrow \,\,\,\,\,{\left( {{{{{1 + i\sqrt 3 } \over 2}} \over {{{1 - i\sqrt 3 } \over 2}}}} \right)^n} = 1$$
<br><br>We know,  $$\omega $$ = $$-$$ $${{1 - i\sqrt 3 } \over 2}$$
<br><br>and $$\omega $$<sup>2</sup> = $$-$$ $${{\left( {1 + i\sqrt 3 } \right)} \over 2}$$
<br><br>$$ \Rightarrow $$ $$\,\,\,\,$$ $${\left( {{{ - {\omega ^2}} \over { - \omega }}} \right)^n} = 1$$
<br><br>$$ \Rightarrow $$ ($$\omega $$)<sup>n</sup> = 1 = $$\omega $$<sup>3</sup>
<br><br>$$ \Rightarrow $$ $$\,\,\,\,$$ n = 3

### Example 3 (Year: 2019)

**Question:**

If $$z = {{\sqrt 3 } \over 2} + {i \over 2}\left( {i = \sqrt { - 1} } \right)$$, 
<br><br>then (1 + iz + z<sup>5</sup> + iz<sup>8</sup>)<sup>9</sup> is equal to :

**Solution:**

$$z = {{\sqrt 3 } \over 2} + {i \over 2}$$
<br><br>$$ \Rightarrow $$ z = $$\cos {\pi  \over 6}$$ + i $$\sin {\pi  \over 6}$$
<br><br>$$ \Rightarrow $$ z = $${e^{i{\pi  \over 6}}}$$
<picture><source media="(max-width: 320px)" srcset="https://imagex.cdn.examgoal.net/7kejek111aprw/e3620b45-06f6-4766-9b64-59a7eb334820/e77a03c0-e08b-11e9-a7bc-b7b08ce8d541/file-7kejek111aprx-320w.jpg"><source media="(max-width: 500px)" srcset="https://imagex.cdn.examgoal.net/7kejek111aprw/e3620b45-06f6-4766-9b64-59a7eb334820/e77a03c0-e08b-11e9-a7bc-b7b08ce8d541/file-7kejek111aprx-500w.jpg"><source media="(max-width: 680px)" srcset="https://imagex.cdn.examgoal.net/7kejek111aprw/e3620b45-06f6-4766-9b64-59a7eb334820/e77a03c0-e08b-11e9-a7bc-b7b08ce8d541/file-7kejek111aprx-680w.jpg"><source media="(max-width: 860px)" srcset="https://imagex.cdn.examgoal.net/7kejek111aprw/e3620b45-06f6-4766-9b64-59a7eb334820/e77a03c0-e08b-11e9-a7bc-b7b08ce8d541/file-7kejek111aprx-860w.jpg"><source media="(max-width: 1040px)" srcset...

### Example 4 (Year: 2019)

**Question:**

Let z<sub>0</sub> be a root of the quadratic equation, x<sup>2</sup> + x + 1 = 0,  If z = 3 + 6iz$$_0^{81}$$ $$-$$ 3iz$$_0^{93}$$, then arg z is equal to : 

**Solution:**

1 + x + x<sup>2</sup> = 0
<br><br>x = $${{ - 1 \pm \sqrt {1 - 4} } \over 2} = {{ - 1 \pm i\sqrt 3 } \over 2}$$
<br><br>z<sub>0</sub> = w, w<sup>2</sup>
<br><br>Now&nbsp;&nbsp;
<br><br>z = 3 + 6iz$$_0^{81}$$ $$-$$ 3iz$$_0^{93}$$
<br><br>z = 3 + 6iw<sup>81</sup> $$-$$ 3iw<sup>93</sup>&nbsp;&nbsp;&nbsp;&nbsp;&nbsp;&nbsp;(w<sup>93</sup> = w<sup>81</sup> = 1)
<br><br>$$ \Rightarrow $$&nbsp;&nbsp;z = 3 + 3i
<br><br>then arg(z) = tan<sup>$$-$$1</sup>$$\left( {{3 \over 3}} \right)$$ = tan<sup>$$-$$1</sup> (1) = $${\pi  \over 4}$$

### Example 5 (Year: 2019)

**Question:**

Let $$z = {\left( {{{\sqrt 3 } \over 2} + {i \over 2}} \right)^5} + {\left( {{{\sqrt 3 } \over 2} - {i \over 2}} \right)^5}.$$ If R(z) and 1(z) respectively denote the real and imaginary parts of z, then :

**Solution:**

$$z = {\left( {{{\sqrt 3  + i} \over 2}} \right)^5} + {\left( {{{\sqrt 3  - i} \over 2}} \right)^5}$$
<br><br>$$z = {\left( {{e^{i\pi /6}}} \right)^5} + {\left( {{e^{ - i\pi /6}}} \right)^5}$$
<br><br>$$ = {e^{i5\pi /6}} + {e^{ - i5\pi /6}}$$
<br><br>$$ = \cos {{5\pi } \over 6} + i{{\sin 5\pi } \over 6} + \cos \left( {{{ - 5\pi } \over 6}} \right) + i\sin \left( {{{ - 5\pi } \over 6}} \right)$$
<br><br>$$ = 2\cos {{5\pi } \over 6} &lt; 0$$
<br><br>$${\rm I}(z) = 0$$ and  $${\mathop{\rm Re}\nolimits} (z) &lt; 0$$
