---
chapter: complex-numbers
topic: cube-roots-of-unity
jee_frequency: 6
years_appeared: [2004, 2005, 2011, 2018, 2020, 2025]
question_count: 7
difficulty: medium
question_types: ['mcq', 'integer']
exams: ['mains']
---

# Complex Numbers: Cube Roots Of Unity

**JEE Frequency**: Appeared in **6 years** (2004 - 2025)

**Question Count**: 7 questions

## Question Types

- **MCQ**: 5 questions
- **INTEGER**: 2 questions

## Difficulty Distribution

- **Medium**: 5 questions
- **Easy**: 2 questions

## Worked Examples

### Example 1 (Year: 2004)

**Question:**

If $$z = x - iy$$ and $${z^{{1 \over 3}}} = p + iq$$, then 
<br><br>$${{\left( {{x \over p} + {y \over q}} \right)} \over {\left( {{p^2} + {q^2}} \right)}}$$ is equal to :

**Solution:**

Given $${z^{{1 \over 3}}} = p + iq$$
<br><br>$$ \Rightarrow $$ z = (p + iq)<sup>3</sup>
<br><br>= p<sup>3</sup> + (iq)<sup>3</sup> +3p(iq)(p + iq)
<br><br>= p<sup>3</sup> - iq<sup>3</sup> +3ip<sup>2</sup>q - 3pq<sup>2</sup>
<br><br>= p(p<sup>2</sup> - 3q<sup>2</sup>) - iq(q<sup>2</sup> - 3p<sup>2</sup>)
<br><br>Given that $$z = x - iy$$
<br><br>$$\therefore$$ $$x - iy$$ = p(p<sup>2</sup> - 3q<sup>2</sup>) - iq(q<sup>2</sup> - 3p<sup>2</sup>)
<br><br>By comparing both sides we get,
<br><br>$${x \over p} = {p^2} - 3{q^2}$$ and $${y \over q} = {q^2} - 3{p^2}$$
<br><br>$$\therefore$$ $${{\left( {{x \over p} + {y \over q}} \right)} \over {\left( {{p^2} + {q^2}} \right)}}$$
<br><br>= $${{{p^2} - 3{q^2} + {q^2} - 3{p^2}} \over {{p^2} + {q^2}}}$$
<br><br>= $${{ - 2{q^2} - 2{p^2}} \over {{p^2} + {q^2}}}$$
<br><br>= $${{ - 2\left( {{q^2} + {p^2}} \right)} \over {{p^2} + {q^2}}}$$
<br><br>= $$-2$$

### Example 2 (Year: 2005)

**Question:**

If the cube roots of unity are 1, $$\omega \,,\,{\omega ^2}$$ then the roots of the equation $${(x - 1)^3}$$ + 8 = 0, are :

**Solution:**

$${\left( {x - 1} \right)^3} + 8 = 0$$
<br><br>$$ \Rightarrow \left( {x - 1} \right) = \left( { - 2} \right){\left( 1 \right)^{1/3}}$$
<br><br>$$ \Rightarrow x - 1 =  - 2\,\,\,$$ or $$\,\,\, - 2\omega \,\,\,\,$$ or $$\,\,\,\, - 2{\omega ^2}$$
<br><br>or $$\,\,\,x =  - 1\,\,\,$$ or $$\,\,\,1 - 2\omega \,\,\,$$ or $$\,\,\,1 - 2{\omega ^2}.$$ 

### Example 3 (Year: 2011)

**Question:**

If $$\omega ( \ne 1)$$ is a cube root of unity, and $${(1 + \omega )^7} = A + B\omega \,$$. Then $$(A,B)$$ equals :

**Solution:**

$${\left( {1 + \omega } \right)^7} = A + B\omega ;\,\,\,\,{\left( { - {\omega ^2}} \right)^7} = A + B\omega $$
<br><br>$$ - {\omega ^2} = A + B\omega ;\,\,\,\,\,\,\,\,\,\,1 + \omega  = A + B\omega $$
<br><br>$$ \Rightarrow A = 1,B = 1.$$ 

### Example 4 (Year: 2018)

**Question:**

If $$\alpha ,\beta  \in C$$ are the distinct roots of the equation
<br>x<sup>2</sup> - x + 1 = 0, then $${\alpha ^{101}} + {\beta ^{107}}$$ is equal to :

**Solution:**

Given equation, 
<br><br>x<sup>2</sup> $$-$$ x + 1 = 0
<br><br>Roots of this equation
<br><br>x = $${{1 \pm \sqrt 3 i} \over 2}$$
<br><br>$$\therefore\,\,\,$$ $$ \propto \, = \,{{1 + \sqrt 3 \,i} \over 2}$$
<br><br>and $$\beta  = \,{{1 - \sqrt 3 \,i} \over 2}$$
<br><br>We know; 
<br><br>$$\omega  = {{ - 1 + \sqrt 3 \,i} \over 2} =  - \left( {{{1 - \sqrt 3 \,i} \over 2}} \right) =  - \beta $$
<br><br>and $${\omega ^2} = {{ - 1 - \sqrt 3 \,i} \over 2} =  - \left( {{{1 + \sqrt 3 \,i} \over 2}} \right) =  -  \propto $$
<br><br>$$\therefore\,\,\,$$ $$ \propto \, =  - {\omega ^2}$$ and $$\beta \, = \, - \omega $$
<br><br>$$\therefore\,\,\,$$ $${ \propto ^{101}} + {\beta ^{107}}$$
<br><br>$$ = {\left( { - {\omega ^2}} \right)^{101}} + {\left( { - \omega } \right)^{107}}$$
<br><br>$$ = {\left( { - 1} \right)^{101}}.{\left( {{\omega ^2}} \right)^{101}} + {\left( { - 1} \right)^{107}}.{\left( \omega  \right)^{107}}$$
<br><br>$$ =  - 1.{\left( {{\omega ^2}} \right)^{101}} - {\omega ^{107}}$$
<br>...

### Example 5 (Year: 2020)

**Question:**

If a and b are real numbers such that<br> $${\left( {2 + \alpha } \right)^4} = a + b\alpha $$ <br>where $$\alpha  = {{ - 1 + i\sqrt 3 } \over 2}$$  then a + b is
equal to :

**Solution:**

$$\alpha  = \omega $$ as given $$\alpha  = {{ - 1 + i\sqrt 3 } \over 2}$$
<br><br>$$ \Rightarrow {(2 + \omega )^4} = a + b\omega \,({\omega ^3} = 1)$$<br><br>$$ \Rightarrow {2^4} + {4.2^3}\omega  + {6.2^2}{\omega ^3} + 4.2.\,{\omega ^3} + {\omega ^4} = a + b\omega $$<br><br>$$ \Rightarrow 16 + 32\omega  + 24{\omega ^2} + 8 + \omega  = a + b\omega $$<br><br>$$ \Rightarrow 24 + 24{\omega ^2} + 33\omega  = a + b\omega $$<br><br><br>$$ \Rightarrow  - 24\omega  + 33\omega  = a + b\omega $$<br><br>$$ \Rightarrow a = 0,\,b = 9$$
