---
chapter: complex-numbers
topic: conjugate-of-complex-numbers
jee_frequency: 6
years_appeared: [2008, 2019, 2020, 2021, 2022, 2023]
question_count: 14
difficulty: medium
question_types: ['mcq', 'integer']
exams: ['mains']
---

# Complex Numbers: Conjugate Of Complex Numbers

**JEE Frequency**: Appeared in **6 years** (2008 - 2023)

**Question Count**: 14 questions

## Question Types

- **MCQ**: 11 questions
- **INTEGER**: 3 questions

## Difficulty Distribution

- **Easy**: 2 questions
- **Medium**: 12 questions

## Worked Examples

### Example 1 (Year: 2008)

**Question:**

The conjugate of a complex number is $${1 \over {i - 1}}$$ then that complex number is :

**Solution:**

$$\left( {{1 \over {i - 1}}} \right) = {1 \over { - i - 1}} = {{ - 1} \over {i + 1}}$$ 

### Example 2 (Year: 2019)

**Question:**

If a &gt; 0 and z = $${{{{\left( {1 + i} \right)}^2}} \over {a - i}}$$,  has magnitude $$\sqrt {{2 \over 5}} $$, then $$\overline z $$ is equal to :

**Solution:**

$$z = {{{{\left( {1 + i} \right)}^2}} \over {a - i}} \times {{a + i} \over {a + i}}$$<br><br>
$$ \Rightarrow z = {{\left( {1 - 1 + 2i} \right)\left( {a + i} \right)} \over {{a^2} + 1}} = {{2ai - 2} \over {{a^2} + 1}}$$  <br><br>
$$ \Rightarrow \left| z \right| = \sqrt {{{\left( {{{ - 2} \over {{a^2} + 1}}} \right)}^2} + {{\left( {{{2a} \over {{a^2} + 1}}} \right)}^2}}  = \sqrt {{{4 + 4{a^2}} \over {{{({a^2} + 1)}^2}}}} $$<br><br>
$$ \Rightarrow \sqrt {{{4(1 + {a^2})} \over {{{({a^2} + 1)}^2}}}}  = {2 \over {\sqrt {{a^2} + 1} }}$$.... (i)<br><br>
Now given $$\left| z \right| = \sqrt {{2 \over 5}} $$<br><br>
so $$\sqrt {{2 \over 5}}  = {2 \over {\sqrt {1 + {a^2}} }}$$ from equation (i)<br><br>
By squaring both sides<br><br>
$$ \Rightarrow {2 \over 5} = {4 \over {1 + {a^2}}}$$<br><br>
$$ \Rightarrow 1 + {a^2} = 10$$<br><br>
a<sup>2</sup> = 9<br><br>
$$ \Rightarrow $$ a = $$ \pm $$ 3 
<br><br>$$ \because $$ (a &gt; 0) then a = 3
<br><br>Now $$\overline z  = {{{{\left( {1 - i} \right)}^2}} ...

### Example 3 (Year: 2020)

**Question:**

If the equation, x<sup>2</sup> + bx + 45 = 0 (b $$ \in $$ R) has
conjugate complex roots and they satisfy
|z +1| = 2$$\sqrt {10} $$ , then :

**Solution:**

x<sup>2</sup>
 + bx = 45 = 0 (b $$ \in $$ R)
<br>has roots $$\alpha $$ + i$$\beta $$, $$\alpha $$ – i$$\beta $$
<br>sum of roots = – b = 2$$\alpha $$
<br>product of roots = 45 = 
$$\alpha $$<sup>2</sup>
 + $$\beta $$<sup>2</sup>
<br><br>Let z = x + iy
<br><br>$$ \therefore $$ |x + iy +1| = 2$$\sqrt {10} $$
<br><br>$${\left| {x + iy + 1} \right|^2} = {\left( {2\sqrt {10} } \right)^2}$$
<br><br>$$ \Rightarrow $$ (x + 1)<sup>2</sup> + y<sup>2</sup> = 40
<br><br>$$ \Rightarrow $$ ($$\alpha $$ + 1)<sup>2</sup> + $$\beta $$<sup>2</sup> = 40
<br><br> [putting real part $$\alpha $$ in place of x and imaginary part $$\beta $$ in place of y]
<br><br>$$ \Rightarrow $$ $$\alpha $$<sup>2</sup> + 2$$\alpha $$ + 1 + $$\beta $$<sup>2</sup> = 40
<br><br>$$ \Rightarrow $$ 45 + 2$$\alpha $$ + 1 = 40
<br><br>$$ \Rightarrow $$ $$\alpha $$ = -3
<br><br>$$ \therefore $$ -b = 2$$\alpha $$ = 2$$ \times $$(-3) = -6
<br><br>$$ \Rightarrow $$ b = 6
<br><br>By checking options we found b<sup>2</sup> – b = 30.

### Example 4 (Year: 2021)

**Question:**

If $$\alpha$$, $$\beta$$ $$\in$$ R are such that 1 $$-$$ 2i (here i<sup>2</sup> = $$-$$1) is a root of z<sup>2</sup> + $$\alpha$$z + $$\beta$$ = 0, then ($$\alpha$$ $$-$$ $$\beta$$) is equal to :

**Solution:**

1 $$-$$ 2i is the root of the equation. So other root is 1 $$+$$ 2i
<br><br>$$ \therefore $$ Sum of roots = 1 $$-$$ 2i + 1 $$+$$ 2i = 2 = -$$\alpha $$
<br><br>Product of roots = (1 $$-$$ 2i)(1 $$+$$ 2i) = 1 - 4i<sup>2</sup> = 5 = $$\beta $$
<br><br>$$ \therefore $$ $$\alpha $$ - $$\beta $$ = -2 - 5 = -7

### Example 5 (Year: 2021)

**Question:**

Let z and $$\omega$$ be two complex numbers such that $$\omega = z\overline z  - 2z + 2,\left| {{{z + i} \over {z - 3i}}} \right| = 1$$ and Re($$\omega$$) has minimum value. Then, the minimum value of n $$\in$$ N for which $$\omega$$<sup>n</sup> is real, is equal to ______________.

**Solution:**

Let z = x + iy<br><br>| z + i | = | z $$-$$ 3i |<br><br>$$ \Rightarrow $$ y = 1<br><br>Now <br><br>$$\omega$$ = x<sup>2</sup> + y<sup>2</sup> $$-$$ 2x $$-$$ 2iy + 2<br><br>$$\omega$$ = x<sup>2</sup> + 1 $$-$$ 2x $$-$$ 2i + 2<br><br>Re($$\omega$$) = x<sup>2</sup> $$-$$ 2x + 3<br><br>Re($$\omega$$) = (x $$-$$ 1)<sup>2</sup> + 2<br><br>Re($$\omega$$)<sub>min</sub> at x = 1 $$ \Rightarrow $$ z = 1 + i<br><br>Now, <br><br>$$\omega$$ = 1 + 1 $$-$$ 2 $$-$$ 2i + 2<br><br>$$\omega$$ = 2(1 $$-$$ i) = 2$$\sqrt 2 {e^{i\left( {{{ - \pi } \over 4}} \right)}}$$<br><br>$$\omega$$<sup>n</sup> = 2$$\sqrt 2 {e^{i\left( {{{ - n\pi } \over 4}} \right)}}$$<br><br>If $$\omega$$<sup>n</sup> is real $$ \Rightarrow $$ n = 4
