---
chapter: differentiation
topic: differentiation-of-a-function-with-respect-to-another-function
jee_frequency: 3
years_appeared: [2018, 2019, 2020]
question_count: 3
difficulty: medium
question_types: ['mcq']
exams: ['mains']
---

# Differentiation: Differentiation Of A Function With Respect To Another Function

**JEE Frequency**: Appeared in **3 years** (2018 - 2020)

**Question Count**: 3 questions

## Question Types

- **MCQ**: 3 questions

## Difficulty Distribution

- **Medium**: 3 questions

## Worked Examples

### Example 1 (Year: 2018)

**Question:**

If $$x = \sqrt {{2^{\cos e{c^{ - 1}}}}} $$ and $$y = \sqrt {{2^{se{c^{ - 1}}t}}} \,\,\left( {\left| t \right| \ge 1} \right),$$ then $${{dy} \over {dx}}$$ is equal to :

**Solution:**

x =  $$\sqrt {{2^{\cos e{c^{ - 1}}t}}} $$
<br><br>$$\therefore\,\,\,\,$$ $${{dx} \over {dt}}$$ = $${1 \over {2\sqrt {{2^{\cos e{c^{ - 1}}t}}} }}$$ $$ \times $$ ($${2^{\cos e{c^{ - 1}}t}}\,.\,\log 2$$) $$ \times $$ $${{ - 1} \over {t\sqrt {{t^2} - 1} }}$$
<br><br>$${{dy} \over {dt}}$$ = $${1 \over {2\sqrt {{2^{{{\sec }^{ - 1}}t}}} }}$$ $$ \times $$ $$\left( {{2^{{{\sec }^{ - 1}}t}}\log 2} \right)$$ $$ \times $$ $${1 \over {t\sqrt {{t^2} - 1} }}$$
<br><br>$$\therefore\,\,\,\,$$ $${{dy} \over {dx}}$$ 
<br><br>= $${{{{dy} \over {dt}}} \over {{{dx} \over {dt}}}}$$
<br><br>= $${{ - \sqrt {{2^{\cos e{c^{ - 1}}t}}} } \over {\sqrt {{2^{\cos e{c^{ - 1}}t}}} }}$$ $$ \times $$ $${{{2^{{{\sec }^{ - 1}}t}}} \over {{2^{\cos e{c^{ - 1}}t}}}}$$
<br><br>= $$ - \sqrt {{{{2^{{{\sec }^{ - 1}}t}}} \over {{2^{\cos e{c^{ - 1}}t}}}}} $$
<br><br>= $$-$$ $${y \over x}$$ 

### Example 2 (Year: 2019)

**Question:**

The derivative of $${\tan ^{ - 1}}\left( {{{\sin x - \cos x} \over {\sin x + \cos x}}} \right)$$, with respect to $${x \over 2}$$
, where $$\left( {x \in \left( {0,{\pi  \over 2}} \right)} \right)$$ is :

**Solution:**

$$y = {\tan ^{ - 1}}\left( {{{\tan x - 1} \over {\tan x + 1}}} \right)$$<br><br>
$$ \Rightarrow $$ $$ - {\tan ^{ - 1}}\left( {{{1 - \tan x} \over {1 + \tan x}}} \right)$$<br><br>
$$ \Rightarrow $$ $$ - {\tan ^{ - 1}}\left( {\tan \left( {{\pi  \over 4} - x} \right)} \right)$$<br><br>
$$ \Rightarrow $$ $$ - \left( {{\pi  \over 4} - x} \right)$$<br><br>
$$ \Rightarrow $$ $${{dy} \over {dx}} = 1$$<br><br>
Now if differentiation of $${x \over 2}$$ w.r.t is $${1 \over 2}$$<br><br>
$$ \Rightarrow $$ So differentiation of y w.r.t $${x \over 2}$$ is $$1 \over {1 \over 2}$$ = 2

### Example 3 (Year: 2020)

**Question:**

The derivative of 
<br>$${\tan ^{ - 1}}\left( {{{\sqrt {1 + {x^2}}  - 1} \over x}} \right)$$ with<br> respect to $${\tan ^{ - 1}}\left( {{{2x\sqrt {1 - {x^2}} } \over {1 - 2{x^2}}}} \right)$$ at x = $${1 \over 2}$$ is :

**Solution:**

Let f = $${\tan ^{ - 1}}\left( {{{\sqrt {1 + {x^2}}  - 1} \over x}} \right)$$
<br><br>Put x = tan $$\theta $$ $$ \Rightarrow $$ $$\theta $$ = tan<sup>–1</sup> x
<br><br>f = $${\tan ^{ - 1}}\left( {{{\sec \theta  - 1} \over {\tan \theta }}} \right)$$
<br><br>$$ \Rightarrow $$ f = $${\tan ^{ - 1}}\left( {{{1 - \cos \theta } \over {\sin \theta }}} \right)$$ = $${\theta  \over 2}$$
<br><br>$$ \Rightarrow $$ f = $${{{{\tan }^{ - 1}}x} \over 2}$$
<br><br>$$ \therefore $$ $${{df} \over {dx}}$$ = $${1 \over {2\left( {1 + {x^2}} \right)}}$$ ....(1)
<br><br>Let g = $${\tan ^{ - 1}}\left( {{{2x\sqrt {1 - {x^2}} } \over {1 - 2{x^2}}}} \right)$$
<br><br>Put x = sin $$\theta $$ $$ \Rightarrow $$ $$\theta $$ = sin<sup>–1</sup>
 x
<br><br>$$ \Rightarrow $$ g = $${\tan ^{ - 1}}\left( {{{2\sin \theta \cos \theta } \over {1 - 2{{\sin }^2}\theta }}} \right)$$
<br><br>$$ \Rightarrow $$ g = tan<sup>–1</sup>
 (tan 2$$\theta $$) = 2$$\theta $$
<br><br>$$ \Rightarrow $$ g = 2sin<sup>-1</sup> x
<br><br>$$ \Righ...
