---
chapter: differential-equations
topic: formation-of-differential-equations
jee_frequency: 9
years_appeared: [2004, 2007, 2009, 2018, 2020, 2021, 2022, 2023, 2024]
question_count: 19
difficulty: medium
question_types: ['mcq', 'integer']
exams: ['mains']
---

# Differential Equations: Formation Of Differential Equations

**JEE Frequency**: Appeared in **9 years** (2004 - 2024)

**Question Count**: 19 questions

## Question Types

- **MCQ**: 16 questions
- **INTEGER**: 3 questions

## Difficulty Distribution

- **Medium**: 18 questions
- **Easy**: 1 questions

## Worked Examples

### Example 1 (Year: 2004)

**Question:**

The differential equation for the family of circle $${x^2} + {y^2} - 2ay = 0,$$ where a is an arbitrary constant is :

**Solution:**

$${x^2} + {y^2} - 2ay = 0\,\,\,\,\,\,\,\,\,\,\,...\left( 1 \right)$$
<br><br>Differentiate, 
<br><br>$$2x + 2y{{dy} \over {dx}} - 2a{{dy} \over {dx}} = 0$$ 
<br><br>$$\,\,\,\,\,\,\,\,\,\,\,\,\,\, \Rightarrow a = {{x + yy'} \over {y'}}$$
<br><br>Put in $$(1),$$ $${x^2} + {y^2} - 2\left( {{{x + yy'} \over {y'}}} \right) = y = 0$$
<br><br>$$ \Rightarrow \left( {{x^2} + {y^2}} \right)y' - 2xy - 2{y^2}y' = 0$$
<br><br>$$ \Rightarrow \left( {{x^2} - {y^2}} \right)y' = 2xy$$

### Example 2 (Year: 2007)

**Question:**

The differential equation of all circles passing through the origin and having their centres on the $$x$$-axis is :

**Solution:**

General equation of circles passing through origin 
<br><br>and having their centres on the $$x$$-axis is 
<br><br>$${x^2} + {y^2} + 2gx = 0\,\,\,\,....\left( i \right)$$
<br><br>On differentiating $$w.r.t.x,$$ we get
<br><br>$$2x + 2y.{{dy} \over {dx}} + 2g = 0$$
<br><br>$$ \Rightarrow g =  - \left( {x + y{{dy} \over {dx}}} \right)$$
<br><br>$$\therefore$$ equation $$(i)$$ be 
<br><br>$${x^2} + {y^2} + 2\left\{ { - \left( {x + y{{dy} \over {dx}}} \right)} \right\}x = 0$$
<br><br>$$ \Rightarrow {x^2} + {y^2} - 2{x^2} - 2x{{dy} \over {dx}}.y = 0$$
<br><br>$$ \Rightarrow {y^2} = {x^2} + 2xy{{dy} \over {dx}}$$

### Example 3 (Year: 2009)

**Question:**

The differential equation which represents the family of curves $$y = {c_1}{e^{{c_2}x}},$$ where $${c_1}$$ , and $${c_2}$$ are arbitrary constants, is 

**Solution:**

We have $$y = {c_1}{e^{{c_2}x}}$$
<br><br>$$ \Rightarrow y' = {c_1}{c_2}{e^{{c_2}x}} = {c_2}y$$
<br><br>$$ \Rightarrow {{y'} \over y} = {c_2}$$
<br><br>$$ \Rightarrow {{y''y\left( {y'} \right){}^2} \over {{y^2}}} = 0$$
<br><br>$$ \Rightarrow y''y = {\left( {y'} \right)^2}$$

### Example 4 (Year: 2018)

**Question:**

The differential equation representing the family of ellipse having foci eith on the x-axis or on the $$y$$-axis, center at the origin and passing through the point (0, 3) is : 

**Solution:**

Equation of ellipse,
<br><br>$${{{x^2}} \over {{a^2}}} + {{{y^2}} \over {{b^2}}} = 1$$
<br><br>As ellipse passes through (0, 3)
<br><br>$$\therefore\,\,\,$$ $${{{0^2}} \over {{a^2}}} + {{{3^2}} \over {{b^2}}} = 1$$
<br><br>$$ \Rightarrow $$ &nbsp;&nbsp; b<sup>2</sup> = 9
<br><br>$$\therefore\,\,\,$$ Equation of ellipse becomes, 
<br><br>$${{{x^2}} \over {{a^2}}} + {{{y^2}} \over 9} = 1$$
<br><br>Differentiating w.r.t &nbsp;&nbsp; x,  we get,
<br><br>$${{2x} \over {a{}^2}}$$ + $${{2y} \over 9}$$ . $${{dy} \over {dx}} = 0$$ 
<br><br>$$ \Rightarrow $$ &nbsp;&nbsp; $${x \over {{a^2}}}$$ = $$-$$ $${y \over 9}.{{dy} \over {da}}$$
<br><br>$$ \Rightarrow $$ &nbsp;&nbsp; $${x \over {{a^2}}} =  - {y \over 9}.y'......$$ (1)
<br><br>We got earlier,
<br><br>$${{{x^2}} \over {{a^2}}} + {{{y^2}} \over 9}$$ = 1
<br><br>$$ \Rightarrow $$&nbsp;&nbsp; $${x \over {{a^2}}}.x + {{{y^2}} \over 9} = 1$$
<br><br>putting value of equation (1) here, 
<br><br>$$  {-{y\,y'} \over 9}.x + {{{y^2}} \over 9} = 1$$
<br...

### Example 5 (Year: 2020)

**Question:**

If $$y = \left( {{2 \over \pi }x - 1} \right) cosec\,x$$  is the solution of the
differential equation, <br><br/>$${{dy} \over {dx}} + p\left( x \right)y = {2 \over \pi } cosec\,x$$,<br><br>
$$0 &lt; x &lt; {\pi  \over 2}$$,  then the function p(x) is equal to :

**Solution:**

$$y = \left( {{2 \over \pi }x - 1} \right) cosec\,x$$
<br>Differentiate w.r.t x
<br><br>$${{dy} \over {dx}} = {2 \over \pi }$$cosec x - $$\left( {{2 \over \pi }x - 1} \right)$$cosec x.cot x
<br><br>$$ \Rightarrow $$ $${{dy} \over {dx}}$$ + $$\left( {{2 \over \pi }x - 1} \right)$$cosec x.cot x = $${2 \over \pi }$$cosec x
<br><br>$$ \Rightarrow $$ $${{dy} \over {dx}}$$ + ycot x = $${2 \over \pi }$$cosec x
<br><br>Compare this differential equation with given differential equation, we get
<br><br>p(x) = cot x
