---
chapter: differentiation
topic: differentiation-of-implicit-function
jee_frequency: 8
years_appeared: [2002, 2003, 2009, 2017, 2018, 2019, 2020, 2023]
question_count: 14
difficulty: medium
question_types: ['mcq', 'integer']
exams: ['mains']
---

# Differentiation: Differentiation Of Implicit Function

**JEE Frequency**: Appeared in **8 years** (2002 - 2023)

**Question Count**: 14 questions

## Question Types

- **MCQ**: 13 questions
- **INTEGER**: 1 questions

## Difficulty Distribution

- **Medium**: 10 questions
- **Easy**: 2 questions
- **Hard**: 2 questions

## Worked Examples

### Example 1 (Year: 2002)

**Question:**

If $$y = {\left( {x + \sqrt {1 + {x^2}} } \right)^n},$$ then $$\left( {1 + {x^2}} \right){{{d^2}y} \over {d{x^2}}} + x{{dy} \over {dx}}$$ is 

**Solution:**

$$y = {\left( {x + \sqrt {1 + {x^2}} } \right)^n}$$
<br><br>$${{dy} \over {dx}} = n{\left( {x + \sqrt {1 + {x^2}} } \right)^{n - 1}}$$
<br><br>$$\,\,\,\,\,\,\,\,\,\,\,\,\,\,\,\,\,\,\left( {1 + {1 \over 2}{{\left( {1 + {x^2}} \right)}^{ - 1/2}}.2x} \right);$$
<br><br>$${{dy} \over {dx}} = n{\left( {x + \sqrt {1 + {x^2}} } \right)^{n - 1}}$$
<br><br>$$\,\,\,\,\,\,\,\,\,\,\,\,\,\,\,\,\,\,{{\left( {\sqrt {1 + {x^2}}  + x} \right)} \over {\sqrt {1 + {x^2}} }}$$
<br><br>$$ = {{n{{\left( {\sqrt {1 + {x^2}}  + x} \right)}^n}} \over {\sqrt {1 + {x^2}} }}$$
<br><br>or $$\sqrt {1 + {x^2}} {{dy} \over {dx}} = ny$$
<br><br>or $$\sqrt {1 + {x^2}} {y_1} = ny$$
<br><br>$$\left( {{y_1} = {{dy} \over {dx}}} \right)$$ 
<br><br>Squaring, $$\left( {1 + {x^2}} \right){y_1}^2 = {n^2}{y^2}$$
<br><br>Differentiating, $$\left( {1 + {x^2}} \right)2{y_1}{y_2} + {y_1}^2.2x$$
<br><br>$$ = {n^2}.2y{y_1}$$
<br><br>or $$\left( {1 + {x^2}} \right){y_2} + x{y_1} = {n^2}y$$


### Example 2 (Year: 2003)

**Question:**

Let  $$f\left( x \right)$$ be a polynomial function of second degree. If $$f\left( 1 \right) = f\left( { - 1} \right)$$ and $$a,b,c$$ are in $$A.P, $$ then $$f'\left( a \right),f'\left( b \right),f'\left( c \right)$$  are in 

**Solution:**

$$f\left( x \right) = a{x^2} + bx + c$$
<br><br>$$f\left( 1 \right) = f\left( { - 1} \right)$$
<br><br>$$ \Rightarrow a + b + c = a - b + c$$
<br><br>or $$b = 0$$
<br><br>$$\therefore$$ $$f\left( x \right) = a{x^2} + c$$ 
<br><br>or $$f'\left( x \right) = 2ax$$
<br><br>Now $$f'\left( a \right);f'\left( b \right);$$
<br><br>and $$f'\left( c \right)$$ are $$2a\left( a \right);2a\left( b \right);2a\left( c \right)$$
<br><br>i.e.$$\,2{a^2},\,2ab,\,2ac.$$
<br><br>$$ \Rightarrow $$ If $$a,b,c$$ are in $$A.P.$$ then
<br><br>$$f'\left( a \right);f'\left( b \right)$$ and 
<br><br>$$f'\left( c \right)$$ are also in $$A.P.$$

### Example 3 (Year: 2009)

**Question:**

Let $$y$$ be an implicit function of $$x$$ defined by $${x^{2x}} - 2{x^x}\cot \,y - 1 = 0$$. Then $$y'(1)$$ equals

**Solution:**

$${x^{2x}} - 2{x^x}\,\cot \,y - 1 = 0$$ 
<br><br>$$ \Rightarrow 2\,\cot \,y = {x^x} - {x^{ - x}}$$
<br><br>$$ \Rightarrow 2\,\cot \,y\, = u - {1 \over u}$$
<br><br>where $$u = {x^x}$$
<br><br>Differentiating both sides with respect to $$x,$$ 
<br><br>we get $$ \Rightarrow  - 2\cos e{c^2}y{{dy} \over {dx}}$$
<br><br>$$ = \left( {1 + {1 \over {{u^2}}}} \right){{du} \over {dx}}$$
<br><br>where $$u = {x^x} \Rightarrow \log \,u = x\,\log \,x$$
<br><br>$$ \Rightarrow {1 \over u}{{du} \over {dx}} = 1 + \log \,x$$
<br><br>$$ \Rightarrow {{du} \over {dx}} = {x^x}\left( {1 + \log \,x} \right)$$
<br><br>$$\therefore$$ We get $$ - 2\cos e{c^2}y{{dy} \over {dx}}$$
<br><br>$$ = \left( {1 + {x^{ - 2x}}} \right){x^x}\left( {1 + \log \,x} \right)$$
<br><br>$$ \Rightarrow {{dy} \over {dx}} = {{\left( {{x^x} + {x^{ - x}}} \right)\left( {1 + \log x} \right)} \over { - 2\left( {1 + {{\cot }^2}y} \right)}}\,\,\,\,\,\,...\left( i \right)$$ 
<br><br>Now when 
<br><br>$$x=1,$$ $${x^{2x}} - 2{x^x}\,\cot \,y - 1...

### Example 4 (Year: 2017)

**Question:**

If y = $${\left[ {x + \sqrt {{x^2} - 1} } \right]^{15}} + {\left[ {x - \sqrt {{x^2} - 1} } \right]^{15}},$$
<br><br> then (x<sup>2</sup> $$-$$ 1) $${{{d^2}y} \over {d{x^2}}} + x{{dy} \over {dx}}$$ is equal to : 

**Solution:**

<p>The given equation is</p>
<p>$$y = {({x^2} + \sqrt {{x^2} - 1} )^{15}} + {(x - \sqrt {{x^2} - 1} )^{15}}$$</p>
<p>Differentiating w.r.t. x, we get</p>
<p>$${{dy} \over {dx}} = 15{(x + \sqrt {{x^2} - 1} )^{14}}\left( {1 + {{1(2x)} \over {2\sqrt {{x^2} - 1} }}} \right) + 15{(x - \sqrt {{x^2} - 1} )^{14}}\left( {1 - {{1(2x)} \over {2\sqrt {{x^2} - 1} }}} \right)$$</p>
<p>Here, we have used the standard differentiatials</p>
<p>$${d \over {dx}}{x^n} = n\,{x^{n - 1}}$$</p>
<p>That is, $${d \over {dx}}(\sqrt {f(x)} ) = {1 \over {2\sqrt {f(x)} }} \times {d \over {dx}}(f(x))$$</p>
<p>Therefore</p>
<p>$${{dy} \over {dx}} = {{15{{(x + \sqrt {{x^2} - 1} )}^{14}}(\sqrt {{x^2} - 1}  + x)} \over {\sqrt {{x^2} - 1} }} + {{15{{(x - \sqrt {{x^2} - 1} )}^{14}}(\sqrt {{x^2} - 1}  - x)} \over {\sqrt {{x^2} - 1} }}$$</p>
<p>$$ \Rightarrow \sqrt {{x^2} - 1} {{dy} \over {dx}} = 15{(x + \sqrt {{x^2} - 1} )^{15}} - 15{(x - \sqrt {{x^2} - 1} )^{15}}$$</p>
<p>Differentiating w.r.t. x, we get</p>
<p>$${{1(2x)} ...

### Example 5 (Year: 2018)

**Question:**

If &nbsp;&nbsp;x<sup>2</sup> + y<sup>2</sup> + sin y = 4, then the value of $${{{d^2}y} \over {d{x^2}}}$$ at the point ($$-$$2,0) is :

**Solution:**

Given, x<sup>2</sup> + y<sup>2</sup>  + sin y = 4
<br><br>After differentiating the above equation &nbsp;w.r.t.x &nbsp;we get
<br><br>2x + 2y $${{dy} \over {dx}}$$ + cos y $${{dy} \over {dx}}$$ = 0 &nbsp;&nbsp;&nbsp;&nbsp;&nbsp;&nbsp;&nbsp;&nbsp; . . . . (1)
<br><br>$$ \Rightarrow $$&nbsp;&nbsp;2x + (2y + cos y) $${{dy} \over {dx}}$$ = 0
<br><br>$$ \Rightarrow $$&nbsp;&nbsp;$${{dy} \over {dx}}$$ = $${{ - 2x} \over {2y + \cos y}}$$
<br><br>At ($$-$$ 2, 0), $${\left( {{{dy} \over {dx}}} \right)_{\left( { - 2,0} \right)}}$$ = $${{ - 2x - 2} \over {2 \times 0 + \cos 0}}$$
<br><br>$$ \Rightarrow $$&nbsp;&nbsp;$${\left( {{{dy} \over {dx}}} \right)_{\left( { - 2,0} \right)}}$$ = $${4 \over {0 + 1}}$$
<br><br>$$ \Rightarrow $$ &nbsp;&nbsp;$${\left( {{{dy} \over {dx}}} \right)_{\left( { - 2,0} \right)}}$$ = 4 &nbsp;&nbsp;&nbsp;&nbsp;&nbsp;&nbsp;&nbsp;&nbsp; . . . . .(2)
<br><br>Again differentiating equation (1) w.r.t&nbsp;&nbsp;to&nbsp;&nbsp;x, we get 
<br><br>2 + 2 $${\left( {{{dy} \over {dx}...
