---
chapter: functions
topic: inverse-functions
jee_frequency: 4
years_appeared: [2018, 2020, 2021, 2023]
question_count: 5
difficulty: medium
question_types: ['mcq']
exams: ['mains']
---

# Functions: Inverse Functions

**JEE Frequency**: Appeared in **4 years** (2018 - 2023)

**Question Count**: 5 questions

## Question Types

- **MCQ**: 5 questions

## Difficulty Distribution

- **Easy**: 2 questions
- **Medium**: 3 questions

## Worked Examples

### Example 1 (Year: 2018)

**Question:**

Let <i> f</i> : A $$ \to $$ B be a function defined as f(x) = $${{x - 1} \over {x - 2}},$$ Where A = <b>R</b> $$-$$ {2} and B = <b>R</b> $$-$$ {1}.  Then &nbsp; <i>f</i> &nbsp; is  : 

**Solution:**

Assume,
<br><br>y = f(x)
<br><br>$$ \Rightarrow $$ y = $${{x - 1} \over {x - 2}}$$
<br><br>$$ \Rightarrow $$ yx - 2y = x - 1
<br><br>$$ \Rightarrow $$ (y - 1)x = 2y - 1
<br><br>$$ \Rightarrow $$ x = $${{2y - 1} \over {y - 1}}$$ = f<sup> -1</sup>(y)
<br><br>As on the given domain the function is invertible and its inverse can be computed as shown above.

### Example 2 (Year: 2020)

**Question:**

The inverse function of
<br><br>f(x) = $${{{8^{2x}} - {8^{ - 2x}}} \over {{8^{2x}} + {8^{ - 2x}}}}$$, x $$ \in $$ (-1, 1), is :

**Solution:**

f(x) = $${{{8^{2x}} - {8^{ - 2x}}} \over {{8^{2x}} + {8^{ - 2x}}}}$$ = y
<br><br>$$ \therefore $$ $${{y + 1} \over {y - 1}} = {{{{2.8}^{2x}}} \over { - {{2.8}^{ - 2x}}}}$$
<br><br>$$ \Rightarrow $$ $${{1 + y} \over {1 - y}}$$ = 8<sup>4x</sup>
<br><br>$$ \Rightarrow $$ $${\log _e}\left( {{{1 + y} \over {1 - y}}} \right)$$ = 4x $${\log _e}8$$
<br><br>$$ \Rightarrow $$ x = $${1 \over {4{{\log }_e}8}}{\log _e}\left( {{{1 + y} \over {1 - y}}} \right)$$
<br><br>$$ \therefore $$ f<sup>-1</sup>(x) = $${1 \over 4}\left( {{{\log }_8}e} \right){\log _e}\left( {{{1 + x} \over {1 - x}}} \right)$$

### Example 3 (Year: 2021)

**Question:**

The inverse of $$y = {5^{\log x}}$$ is :

**Solution:**

$$y = {5^{\log x}}$$<br><br>$$ \Rightarrow \log y = \log x.log5$$<br><br>$$ \Rightarrow \log x = {{\log y} \over {\log 5}} = {\log _5}y$$<br><br>$$ \Rightarrow x = {e^{{{\log }_5}y}}$$<br><br>$$ \Rightarrow x = {y^{{{\log }_5}e}}$$<br><br>$$ \Rightarrow x = {y^{{1 \over {\log 5}}}}$$

### Example 4 (Year: 2021)

**Question:**

Let f : R $$-$$ {3} $$ \to $$ R $$-$$ {1} be defined by f(x) = $${{x - 2} \over {x - 3}}$$.<br><br>Let g : R $$ \to $$ R be given as g(x) = 2x $$-$$ 3. Then, the sum of all the values of x for which f<sup>$$-$$1</sup>(x) + g<sup>$$-$$1</sup>(x) = $${{13} \over 2}$$ is equal to :

**Solution:**

Finding inverse of f(x)<br><br>$$y = {{x - 2} \over {x - 3}} \Rightarrow xy - 3y = x - 2 \Rightarrow x(y - 1) = 3y - 2$$<br><br>$$ \therefore $$ $${f^{ - 1}}(x) = {{3x - 2} \over {x - 1}}$$<br><br>Similarly for $${g^{ - 1}}(x)$$<br><br>$$y = 2x - 3 \Rightarrow x = {{y + 3} \over 2} \Rightarrow {g^{ - 1}}(x) = {{x + 3} \over 2}$$<br><br>$$ \therefore $$ $${{3x - 2} \over {x - 1}} + {{x + 3} \over 2} = {{13} \over 2}$$<br><br>$$ \Rightarrow 6x - 4 + {x^2} + 2x - 3 = 13x - 13$$<br><br>$$ \Rightarrow {x^2} - 5x + 6 = 0$$<br><br>$$ \Rightarrow (x - 2)(x - 3) = 0$$<br><br>$$ \Rightarrow $$ x = 2 or 3

### Example 5 (Year: 2023)

**Question:**

<p>The range of $$f(x)=4 \sin ^{-1}\left(\frac{x^{2}}{x^{2}+1}\right)$$ is</p>

**Solution:**

$$
\begin{aligned}
& \frac{x^2}{1+x^2}=1-\frac{1}{1+x^2}<1 \\\\
\therefore & 0 \leq \frac{x^2}{1+x^2}<1 \\\\
\Rightarrow & 0 \leq \sin ^{-1}\left(\frac{x^2}{1+x^2}\right)<\frac{\pi}{2} \\\\
\Rightarrow & 0 \leq 4 \sin ^{-1}\left(\frac{x^2}{1+x^2}\right)<2 \pi
\end{aligned}
$$
