---
chapter: hyperbola
topic: common-tangent
jee_frequency: 3
years_appeared: [2019, 2020, 2022]
question_count: 4
difficulty: medium
question_types: ['mcq', 'integer']
exams: ['mains']
---

# Hyperbola: Common Tangent

**JEE Frequency**: Appeared in **3 years** (2019 - 2022)

**Question Count**: 4 questions

## Question Types

- **MCQ**: 2 questions
- **INTEGER**: 2 questions

## Difficulty Distribution

- **Medium**: 4 questions

## Worked Examples

### Example 1 (Year: 2019)

**Question:**

Equation of a common tangent to the parabola y<sup>2</sup> = 4x and the hyperbola xy = 2 is :

**Solution:**

Let the equation of tangent to parabola
<br><br>y<sup>2</sup> = 4x  be  y = mx + $${1 \over m}$$
<br><br>It is also a tangent to hyperbola xy = 2
<br><br>$$ \Rightarrow $$&nbsp;&nbsp;x$$\left( {mx + {1 \over m}} \right)$$ = 2
<br><br>$$ \Rightarrow $$&nbsp;&nbsp;x<sup>2</sup>m + $${x \over m}$$ $$-$$ 2 = 0
<br><br>D = 0 $$ \Rightarrow $$&nbsp;&nbsp; m = $$-$$ $${1 \over 2}$$
<br><br>So tangent is 2y + x + 4 = 0

### Example 2 (Year: 2020)

**Question:**

If the line y = mx + c is a common tangent to
the hyperbola
<br>$${{{x^2}} \over {100}} - {{{y^2}} \over {64}} = 1$$ and the circle
x<sup>2</sup>
 + y<sup>2</sup>
 = 36, then which one of the following is
true?

**Solution:**

$${{{x^2}} \over {100}} - {{{y^2}} \over {64}} = 1$$
<br><br>$$ \therefore $$ c = $$ \pm $$ $$\sqrt {{a^2}{m^2} - {b^2}} $$
<br><br>$$ \Rightarrow $$ c = $$ \pm $$ $$\sqrt {100{m^2} - 64} $$
<br><br>General tangent to hyperbola in slope form is
<br><br>y = mx $$ \pm $$ $$\sqrt {100{m^2} - 64} $$
<br><br>This tangent is also tangent to the circle x<sup>2</sup>
 + y<sup>2</sup>
 = 36, whose center (0, 0) and radius = 6.
<br><br>Distance of the tangent from the center is
<br><br>$$\left| {{{\sqrt {100{m^2} - 64} } \over {\sqrt {{m^2} + 1} }}} \right|$$ = 6
<br><br>$$ \Rightarrow $$ 100m<sup>2</sup>
 â€” 64 = 36m<sup>2</sup>
 + 36
<br><br>$$ \Rightarrow $$ 64m<sup>2</sup>
 = 100
<br><br>$$ \Rightarrow $$ m = $${{10} \over 8}$$
<br><br>$$ \therefore $$ c<sup>2</sup> = 100 $$ \times $$ $${{100} \over {64}}$$ - 64
<br><br>$$ \Rightarrow $$ c<sup>2</sup> = $${{{{100}^2} - {{64}^2}} \over {64}}$$
<br><br>$$ \Rightarrow $$ c<sup>2</sup> = $${{164 \times 36} \over {64}}$$
<br><br>$$ \Rightarrow $$ ...

### Example 3 (Year: 2022)

**Question:**

<p>A common tangent $$\mathrm{T}$$ to the curves $$\mathrm{C}_{1}: \frac{x^{2}}{4}+\frac{y^{2}}{9}=1$$ and $$C_{2}: \frac{x^{2}}{42}-\frac{y^{2}}{143}=1$$ does not pass through the fourth quadrant. If $$\mathrm{T}$$ touches $$\mathrm{C}_{1}$$ at $$\left(x_{1}, y_{1}\right)$$ and $$\mathrm{C}_{2}$$ at $$\left(x_{2}, y_{2}\right)$$, then $$\left|2 x_{1}+x_{2}\right|$$ is equal to ______________.</p>

**Solution:**

<p>Equation of tangent to ellipse $${{{x^2}} \over 4} + {{{y^2}} \over 9} = 1$$ and given slope m is : $$y = mx + \sqrt {4{m^2} + 9} $$ ..... (i)</p>
<p>For slope m equation of tangent to hyperbola is :</p>
<p>$$y = mx + \sqrt {42{m^2} - 143} $$ ....... (ii)</p>
<p>Tangents from (i) and (ii) are identical then</p>
<p>$$4{m^2} + 9 = 42{m^2} - 143$$</p>
<p>$$\therefore$$ $$m = \, \pm \,2$$ (+2 is not acceptable)</p>
<p>$$\therefore$$ $$m =  - 2$$.</p>
<p>Hence, $${x_1} = {8 \over 5}$$ and $${x_2} = {{84} \over 5}$$</p>
<p>$$\therefore$$ $$|2{x_1} + {x_2}| = \left| {{{16} \over 5} + {{84} \over 5}} \right| = 20$$</p>

### Example 4 (Year: 2022)

**Question:**

<p>For the hyperbola $$\mathrm{H}: x^{2}-y^{2}=1$$ and the ellipse $$\mathrm{E}: \frac{x^{2}}{\mathrm{a}^{2}}+\frac{y^{2}}{\mathrm{~b}^{2}}=1$$, a $$>\mathrm{b}>0$$, let the</p>
<p>(1) eccentricity of $$\mathrm{E}$$ be reciprocal of the eccentricity of $$\mathrm{H}$$, and</p>
<p>(2) the line $$y=\sqrt{\frac{5}{2}} x+\mathrm{K}$$ be a common tangent of $$\mathrm{E}$$ and $$\mathrm{H}$$.</p>
<p>Then $$4\left(\mathrm{a}^{2}+\mathrm{b}^{2}\right)$$ is equal to _____________.</p>

**Solution:**

<p>The equation of tangent to hyperbola $${x^2} - {y^2} = 1$$ within slope $$m$$ is equal to $$y = mx\, \pm \,\sqrt {{m^2} - 1} $$ ...... (i)</p>
<p>And for same slope $$m$$, equation of tangent to ellipse $${{{x^2}} \over {{a^2}}} + {{{y^2}} \over {{b^2}}} = 1$$ is $$y = mx\, \pm \,\sqrt {{a^2}{m^2} + {b^2}} $$ ...... (ii)</p>
<p>$$\because$$ Equation (i) and (ii) are identical</p>
<p>$$\therefore$$ $${a^2}{m^2} + {b^2} = {m^2} - 1$$</p>
<p>$$\therefore$$ $${m^2} = {{1 + {b^2}} \over {1 - {a^2}}}$$</p>
<p>But equation of common tangent is $$y = \sqrt {{5 \over 2}} x + k$$</p>
<p>$$\therefore$$ $$m = \sqrt {{5 \over 2}}  \Rightarrow {5 \over 2} = {{1 + {b^2}} \over {1 - {a^2}}}$$</p>
<p>$$\therefore$$ $$5{a^2} + 2{b^2} = 3$$ ....... (i)</p>
<p>eccentricity of ellipse $$ = {1 \over {\sqrt 2 }}$$</p>
<p>$$\therefore$$ $$1 - {{{b^2}} \over {{a^2}}} = {1 \over 2}$$</p>
<p>$$ \Rightarrow {a^2} = 2{b^2}$$ ....... (ii)</p>
<p>From equation (i) and (ii) : $${a^2} = {1 \over 2},\,{b^2} = {1 \ov...
