---
chapter: quadratic-equation-and-inequalities
topic: range-of-quadratic-expression
jee_frequency: 4
years_appeared: [2006, 2016, 2019, 2024]
question_count: 4
difficulty: medium
question_types: ['mcq', 'integer']
exams: ['mains']
---

# Quadratic Equation And Inequalities: Range Of Quadratic Expression

**JEE Frequency**: Appeared in **4 years** (2006 - 2024)

**Question Count**: 4 questions

## Question Types

- **MCQ**: 3 questions
- **INTEGER**: 1 questions

## Difficulty Distribution

- **Medium**: 3 questions
- **Hard**: 1 questions

## Worked Examples

### Example 1 (Year: 2006)

**Question:**

If $$x$$ is real, the maximum value of $${{3{x^2} + 9x + 17} \over {3{x^2} + 9x + 7}}$$ is 

**Solution:**

$$y = {{3{x^2} + 9x + 17} \over {3{x^2} + 9x + 7}}$$
<br><br>$$3{x^2}\left( {y - 1} \right) + 9x\left( {y - 1} \right) + 7y - 17 = 0$$
<br><br>$$D \ge 0$$ as $$x$$ is real
<br><br>$$81{\left( {y - 1} \right)^2} - 4 \times 3\left( {y - 1} \right)\left( {7y - 17} \right) \ge 0$$
<br><br>$$ \Rightarrow \left( {y - 1} \right)\left( {y - 41} \right) \le 0$$
<br><br>$$ \Rightarrow 1 \le y \le 41$$
<br><br>$$\therefore$$ Max value of $$y$$ is $$41$$ 

### Example 2 (Year: 2016)

**Question:**

The sum of all real values of $$x$$ satisfying the equation $${\left( {{x^2} - 5x + 5} \right)^{{x^2} + 4x - 60}}\, = 1$$ is : 

**Solution:**

Given equation,
$${\left( {{x^2} - 5x + 5} \right)^{{x^2} + 4x - 60}} = 1$$
<br><br><b>Case 1 : </b>When x<sup>2</sup> - 5x + 5 = 1 and x<sup>2</sup> + 4x - 60 is any real no then this equation satisfy.
<br><b>Note :</b> When we put any real number as a power of 1 the value stays always 1 (1<sup> any real no</sup> = 1).
<br> x<sup>2</sup> - 5x + 5 = 1
<br>(x - 1)(x - 4) = 0
<br>$$\therefore$$ x = 1, 4
<br><br><b>Case 2 : </b>When x<sup>2</sup> - 5x + 5 is a real no and x<sup>2</sup> + 4x - 60 = 0 then the given equation satisfy. As we know if power of any real no is zero then it will become 1((any real number)<sup>0</sup> = 1).
<br>For, x<sup>2</sup> + 4x - 60 = 0
<br>(x - 6)(x + 10) = 0
<br>$$\therefore$$ x = 6, -10
<br><br><b>Case 3 :</b> When x<sup>2</sup> - 5x + 5 = -1 and x<sup>2</sup> + 4x - 60 is even this equation satisfy. As we know (-1)<sup>even</sup> = 1.
<br>For, x<sup>2</sup> - 5x + 5 = -1
<br>(x - 2)(x - 3) = 0
<br>$$\therefore$$ x = 2, 3
<br>But x can't be 3 because when...

### Example 3 (Year: 2019)

**Question:**

The number of integral values of m for which the quadratic expression, (1 + 2m)x<sup>2</sup> â€“ 2(1 + 3m)x + 4(1 + m), x $$ \in $$ R, is always positive, is :

**Solution:**

Expression is always positive it
<br><br>2m + 1 &gt; 0 $$ \Rightarrow $$  m &gt; $$-$$ $${1 \over 2}$$  &amp;
<br><br>D &lt; 0 $$ \Rightarrow $$  m<sup>2</sup> $$-$$ 6m $$-$$ 3 &lt; 0
<br><br>&nbsp;&nbsp;&nbsp;&nbsp;&nbsp;&nbsp;3 $$-$$ $$\sqrt {12} $$ &lt; m &lt; 3 + $$\sqrt {12} $$ . . . . (iii)
<br><br>$$ \therefore $$&nbsp;&nbsp;Common interval is 
<br><br>3 $$-$$ $$\sqrt {12} $$ &lt; m &lt; 3 + $$\sqrt {12} $$
<br><br>$$ \therefore $$&nbsp;&nbsp;Intgral value of m {0, 1, 2, 3, 4, 5, 6}

### Example 4 (Year: 2024)

**Question:**

<p>Let $$a, b, c$$ be the lengths of three sides of a triangle satistying the condition $$\left(a^2+b^2\right) x^2-2 b(a+c) x+\left(b^2+c^2\right)=0$$. If the set of all possible values of $$x$$ is the interval $$(\alpha, \beta)$$, then $$12\left(\alpha^2+\beta^2\right)$$ is equal to __________.</p>

**Solution:**

<p>$$\left(a^2+b^2\right) x^2-2 b(a+c) x+b^2+c^2=0$$</p>
<p>$$\begin{aligned}
& \Rightarrow a^2 x^2-2 a b x+b^2+b^2 x^2-2 b c x+c^2=0 \\
& \Rightarrow(a x-b)^2+(b x-c)^2=0 \\
& \Rightarrow a x-b=0, \quad b x-c=0 \\
& \Rightarrow a+b>c \quad b+c>a \quad c+a>b
\end{aligned}$$</p>
<p>$$\begin{array}{l|l|l}
a+a x>b x & a x+b x>a & a x^2+a>a x \\
a+a x>a x^2 & a x+a x^2>a & x^2-x+1>0 \\
x^2-x-1<0 & x^2+x-1>0 & \text { always true }
\end{array}$$</p>
<p>$$\begin{aligned}
& \frac{1-\sqrt{5}}{2}< x<\frac{1+\sqrt{5}}{2} \\
& x< \frac{-1-\sqrt{5}}{2}, \text { or } x >\frac{-1+\sqrt{5}}{2}
\end{aligned}$$</p>
<p>$$\begin{aligned}
& \Rightarrow \frac{\sqrt{5}-1}{2}< x<\frac{\sqrt{5}+1}{2} \\
& \Rightarrow \alpha=\frac{\sqrt{5}-1}{2}, \beta=\frac{\sqrt{5}+1}{2} \\
& 12\left(\alpha^2+\beta^2\right)=12\left(\frac{(\sqrt{5}-1)^2+(\sqrt{5}+1)^2}{4}\right)=36
\end{aligned}$$</p>
