---
chapter: quadratic-equation-and-inequalities
topic: common-roots
jee_frequency: 9
years_appeared: [2004, 2008, 2013, 2016, 2019, 2020, 2021, 2022, 2023]
question_count: 10
difficulty: medium
question_types: ['mcq', 'integer']
exams: ['mains']
---

# Quadratic Equation And Inequalities: Common Roots

**JEE Frequency**: Appeared in **9 years** (2004 - 2023)

**Question Count**: 10 questions

## Question Types

- **MCQ**: 7 questions
- **INTEGER**: 3 questions

## Difficulty Distribution

- **Easy**: 1 questions
- **Medium**: 7 questions
- **Hard**: 2 questions

## Worked Examples

### Example 1 (Year: 2004)

**Question:**

If one root of the equation $${x^2} + px + 12 = 0$$  is 4, while the equation $${x^2} + px + q = 0$$ has equal roots, 
<br>then the value of $$'q'$$ is 

**Solution:**

$$4$$ is a root of $${x^2} + px + 12 = 0$$
<br><br>$$ \Rightarrow 16 + 4p + 12 = 0$$
<br><br>$$ \Rightarrow p =  - 7$$
<br><br>Now, the equation $${x^2} + px + q = 0$$
<br><br>has equal roots. 
<br><br>$$\therefore$$ $${p^2} - 4q = 0$$ $$ \Rightarrow q = {{{p^2}} \over 4} = {{49} \over 4}$$

### Example 2 (Year: 2008)

**Question:**

The quadratic equations $${x^2} - 6x + a = 0$$ and $${x^2} - cx + 6 = 0$$ have one root in common. The other roots of the first and second equations are integers in the ratio 4 : 3. Then the common root is 

**Solution:**

Let the roots of equation $${x^2} - 6x + a = 0$$ be $$\alpha $$ 
<br><br>and $$4$$ $$\beta $$ and that of the equation 
<br><br>$${x^2} - cx + 6 = 0$$ be $$\alpha $$ and $$3\beta .$$ Then
<br><br>$$\,\,\,\,\,\,\,\,\,\,\,\,\,\,\,\,\,\,\,\,\,\,\,\alpha  + 4\beta  = 6;\,\,\,\,\,\,\,4\alpha \beta  = a$$
<br><br>and $$\,\,\,\,\,\,\,\,\,\,\,\,\,\alpha  + 3\beta  = c;\,\,\,\,\,\,\,3\alpha \beta  = 6$$
<br><br>$$ \Rightarrow \,\,\,\,\,\,\,\,\,\,\,\,\,\,\,a = 8$$
<br><br>$$\therefore$$ The equation becomes 
<br><br>$${x^2} - 6x + 8 = 0$$
<br><br>$$ \Rightarrow \left( {x - 2} \right)\left( {x - 4} \right) = 0$$
<br><br>$$ \Rightarrow $$ roots are $$2$$ and $$4$$
<br><br>$$ \Rightarrow \alpha  = 2,\beta  = 1$$
<br><br>$$\therefore$$ Common root is $$2.$$

### Example 3 (Year: 2013)

**Question:**

If the equations $${x^2} + 2x + 3 = 0$$ and $$a{x^2} + bx + c = 0,$$ $$a,\,b,\,c\, \in \,R,$$  have a common root, then $$a\,:b\,:c\,$$ is 

**Solution:**

Given equations are 
<br><br>$$\,\,\,\,\,\,\,\,\,\,\,\,{x^2} + 2x + 3 = 0\,\,\,\,\,...\left( i \right)$$
<br><br>$$\,\,\,\,\,\,\,\,\,\,\,\,a{x^2} + bx + c = 0\,\,\,...\left( {ii} \right)$$
<br><br>Roots of equation $$(i)$$  are imaginary roots.
<br><br>According to the question $$(ii)$$ will also have both roots same as $$(i).$$ 
<br><br>Thus $${a \over 1} = {b \over 2} = {c \over 3} = \lambda \left( {say} \right)$$
<br><br>$$ \Rightarrow a = \lambda ,b = 2\lambda ,c = 3\lambda $$
<br><br>Hence, required ratio is $$1:2:3$$ 

### Example 4 (Year: 2016)

**Question:**

If the equations x<sup>2</sup> + bx−1 = 0 and x<sup>2</sup> + x + b = 0 have a common root different from −1, then $$\left| b \right|$$ is equal to :

**Solution:**

Given,
<br><br>x<sup>2</sup> + bx $$-$$ 1 = 0 . . . . .(1)
<br><br>and x<sup>2</sup> + x + b = 0 . . . . . (2)
<br><br>Performing (1) $$-$$ (2) we get, 
<br><br>bx $$-$$ 1 $$-$$ x $$-$$ b = 0
<br><br>$$ \Rightarrow $$&nbsp;&nbsp;&nbsp; x(b $$-$$ 1) = b + 1
<br><br>$$ \Rightarrow $$&nbsp;&nbsp;&nbsp;x = $${{b + 1} \over {b - 1}}$$
<br><br>putting value of x in equation (2),
<br><br>$${\left( {{{b + 1} \over {b - 1}}} \right)^2} + \left( {{{b + 1} \over {b - 1}}} \right) + b = 0$$
<br><br>$$ \Rightarrow $$&nbsp;&nbsp;&nbsp;(b + 1)<sup>2</sup> + (b + 1) (b $$-$$ 1) + b (b $$-$$ 1)<sup>2</sup> = 0
<br><br>$$ \Rightarrow $$&nbsp;&nbsp;&nbsp; b<sup>2</sup> + 2b + 1 + b<sup>2</sup> $$-$$ 1 + b (b<sup>2</sup> $$-$$ 2b + 1) = 0
<br><br>$$ \Rightarrow $$&nbsp;&nbsp;&nbsp; 2b<sup>3</sup> + 2b + b<sup>3</sup> $$-$$ 2b<sup>2</sup>  + b = 0
<br><br>$$ \Rightarrow $$ &nbsp;&nbsp;&nbsp; b<sup>3</sup> + 3b = 0
<br><br>$$ \Rightarrow $$&nbsp;&nbsp;&nbsp; b(b<sup>2</sup> + 3) = 0
<br><br>b<sup>2</sup> = ...

### Example 5 (Year: 2019)

**Question:**

If $$\alpha $$, $$\beta $$ and $$\gamma $$ are three consecutive terms of a non-constant G.P. such that the equations $$\alpha $$x
<sup>2</sup>
 + 2$$\beta $$x + $$\gamma $$ = 0 and
x<sup>2</sup>
 + x – 1 = 0 have a common root, then $$\alpha $$($$\beta $$ + $$\gamma $$) is equal to : 

**Solution:**

Let the common ratio of G.P is <b>r</b><br><br>
Then the equation of  $$\alpha {x^2} + 2\beta x + \gamma  = 0$$<br><br>
$$ \Rightarrow $$ $$\alpha {x^2} + 2\alpha rx + \alpha {r^2} = 0$$<br><br>
$$ \Rightarrow $$ x<sup>2</sup> + 2rx + r<sup>2</sup> = 0 ........<b>(i)</b><br>
Equation (i) and x<sup>2</sup> + x - 1 = 0 ......... <b>(ii)</b> has a common root.<br><br>
Now (i) - (ii) $$ \Rightarrow $$ (2r-1)x + (r<sup>2</sup>+1) = 0<br><br>
$$ \Rightarrow $$ x = $${{ - \left( {{r^2} + 1} \right)} \over {2r - 1}}$$ ....... <b>(iii)</b><br><br>
Now putting (iii) in equation (ii) <br><br>
$$ \Rightarrow $$ (r<sup>2</sup>+1)<sup>2</sup> - (r<sup>2</sup>+1) (2r - 1) -  (2r - 1)<sup>2</sup> = 0<br><br>
$$ \Rightarrow $$ r<sup>4</sup> - 2r<sup>3</sup> - r<sup>2</sup> + 2r + 1 = 0 ..........<b> (iv)</b><br><br>
dividing equation (iv) by r<sup>2</sup><br><br>
$$ \Rightarrow $$ r<sup>2</sup> - 2r - 1 + $${2 \over r} + {1 \over {{r^2}}} = 0$$<br><br>
$$ \Rightarrow $$ $${\left( {r - {1 \over r}} \rig...
