---
chapter: quadratic-equation-and-inequalities
topic: inequalities
jee_frequency: 6
years_appeared: [2002, 2008, 2019, 2021, 2022, 2024]
question_count: 8
difficulty: medium
question_types: ['mcq', 'integer']
exams: ['mains']
---

# Quadratic Equation And Inequalities: Inequalities

**JEE Frequency**: Appeared in **6 years** (2002 - 2024)

**Question Count**: 8 questions

## Question Types

- **MCQ**: 7 questions
- **INTEGER**: 1 questions

## Difficulty Distribution

- **Easy**: 1 questions
- **Medium**: 7 questions

## Worked Examples

### Example 1 (Year: 2002)

**Question:**

If $$a,\,b,\,c$$ are distinct $$ + ve$$ real numbers and $${a^2} + {b^2} + {c^2} = 1$$ then $$ab + bc + ca$$ is 

**Solution:**

As $$\,\,\,\,\,{\left( {a - b} \right)^2} + {\left( {b - c} \right)^2} + {\left( {c - a} \right)^2} &gt; 0$$
<br><br>$$ \Rightarrow 2\left( {{a^2} + {b^2} + {c^2} - ab - bc - ca} \right) &gt; 0$$
<br><br>$$ \Rightarrow 2 &gt; 2\left( {ab + bc + ca} \right)$$
<br><br>$$ \Rightarrow ab + bc + ca &lt; 1$$

### Example 2 (Year: 2008)

**Question:**

<b>STATEMENT - 1 :</b> For every natural number $$n \ge 2,$$ 
$$${1 \over {\sqrt 1 }} + {1 \over {\sqrt 2 }} + ........ + {1 \over {\sqrt n }} &gt; \sqrt n .$$$
<p><b>STATEMENT - 2 :</b> For every natural number  $$n \ge 2,$$, 
$$$\sqrt {n\left( {n + 1} \right)}  &lt; n + 1.$$$</p>


**Solution:**

Statements $$2$$ is  $$\sqrt {n\left( {n + 1} \right)}  &lt; n + 1,n \ge 2$$
<br><br>$$ \Rightarrow \sqrt n  &lt; \sqrt {n + 1} ,n \ge 2$$ which is true
<br><br>$$ \Rightarrow \sqrt 2  &lt; \sqrt 3  &lt; \sqrt 4  &lt; \sqrt 5  &lt;  -  -  -  -  -  - \sqrt n $$
<br><br>Now $$\sqrt 2  &lt; \sqrt n  \Rightarrow {1 \over {\sqrt 2 }} &gt; {1 \over {\sqrt n }}$$
<br><br>$$\sqrt 3  &lt; \sqrt n  \Rightarrow {1 \over {\sqrt 3 }} &gt; {1 \over {\sqrt n }};$$ 
<br><br>$$\sqrt n  \le \sqrt n  \Rightarrow {1 \over {\sqrt n }} \ge {1 \over {\sqrt n }}$$
<br><br>Also $${1 \over {\sqrt 1 }} &gt; {1 \over {\sqrt n }}$$ 
<br><br>$$\therefore$$ Adding all, we get 
<br><br>$${1 \over {\sqrt 1 }} + {1 \over {\sqrt 2 }} + {1 \over {\sqrt 3 }} + ....... + {1 \over n} &gt; {n \over {\sqrt n }} = \sqrt n $$
<br><br>Hence both the statements are correct and statement $$2$$ is a correct explanation of statement $$-1.$$ 

### Example 3 (Year: 2019)

**Question:**

All the pairs (x, y) that satisfy the inequality
<br>$${2^{\sqrt {{{\sin }^2}x - 2\sin x + 5} }}.{1 \over {{4^{{{\sin }^2}y}}}} \le 1$$
<br>also satisfy the equation

**Solution:**

$${2^{\sqrt {{{\sin }^2}x - 2\sin x + 5} }} \le {2^{2{{\sin }^2}y}}$$<br><br>
$$ \Rightarrow $$ $$\sqrt {{{\sin }^2}x - 2\sin x + 5}  \le 2{\sin ^2}y$$<br><br>
$$ \Rightarrow \sqrt {{{\left( {\sin x - 1} \right)}^2} + 4}  \le 2{\sin ^2}y$$<br><br>
it is true when sinx = 1, |siny| = 1<br><br>
so sinx = |siny|


### Example 4 (Year: 2021)

**Question:**

Let p and q be two positive numbers such that p + q = 2 and p<sup>4</sup>+q<sup>4</sup> = 272. Then p and q are
roots of the equation :

**Solution:**

$${p^2} + {q^2} = {(p + q)^2} - 2pq$$<br><br>$$ = 4 - 2pq$$<br><br>Now, $${\left( {{p^2} + {q^2}} \right)^2} = {p^4} + {q^4} + 2{p^2}{q^2}$$<br><br>$$ \Rightarrow {\left( {4 - 2pq} \right)^2} = 272 + 2{p^2}{q^2}$$<br><br>$$ \Rightarrow 16 + 4{p^2}{q^2} - 16pq = 272 + 2{p^2}{q^2}$$<br><br>$$ \Rightarrow 2{p^2}{q^2} - 16pq - 256 = 0$$<br><br>$$ \Rightarrow {p^2}{q^2} - 8pq - 128 = 0$$<br><br>$$ \Rightarrow (pq - 16)(pq + 8) = 0$$<br><br>$$ \Rightarrow pq = 16, - 8$$
<br/><br/>Here, pq = - 8 is not possible as p and q are positive.
<br/><br/>$$ \therefore $$ pq = 16
<br/><br/>Now, the equation whose roots are p and q is
<br><br>$${x^2} - 2x + 16 = 0$$

### Example 5 (Year: 2021)

**Question:**

The integer 'k', for which the inequality x<sup>2</sup> $$-$$ 2(3k $$-$$ 1)x + 8k<sup>2</sup> $$-$$ 7 &gt; 0 is valid for every x in R, is :

**Solution:**

$${x^2} - 2(3k - 1)x + 8{k^2} - 7 &gt; 0$$<br><br>Now, D &lt; 0<br><br>$$ \Rightarrow 4{(3k - 1)^2} - 4 \times 1 \times (8{k^2} - 7) &lt; 0$$<br><br>$$ \Rightarrow 9{k^2} - 6k + 1 - 8{k^2} + 7 &lt; 0$$<br><br>$$ \Rightarrow {k^2} - 6k + 8 &lt; 0$$<br><br>$$ \Rightarrow (k - 4)(k - 2) &lt; 0$$<br><br>2 &lt; k &lt; 4
<br><br>then k = 3
