---
chapter: sequences-and-series
topic: harmonic-progression
jee_frequency: 4
years_appeared: [2005, 2006, 2022, 2025]
question_count: 4
difficulty: medium
question_types: ['mcq']
exams: ['mains']
---

# Sequences And Series: Harmonic Progression

**JEE Frequency**: Appeared in **4 years** (2005 - 2025)

**Question Count**: 4 questions

## Question Types

- **MCQ**: 4 questions

## Difficulty Distribution

- **Medium**: 4 questions

## Worked Examples

### Example 1 (Year: 2005)

**Question:**

If $$x = \sum\limits_{n = 0}^\infty  {{a^n},\,\,y = \sum\limits_{n = 0}^\infty  {{b^n},\,\,z = \sum\limits_{n = 0}^\infty  {{c^n},} } } \,\,$$ where a, b, c are in A.P and $$\,\left| a \right| &lt; 1,\,\left| b \right| &lt; 1,\,\left| c \right| &lt; 1$$ then x, y, z are in 

**Solution:**

$$x = \sum\limits_{n = 0}^\infty  {{a^n}}  = {1 \over {1 - a}}\,\,\,\,\,\,\,\,\,\,a = 1 - {1 \over x}$$
<br><br>$$y = \sum\limits_{n = 0}^\infty  {{b^n}}  = {1 \over {1 - b}}\,\,\,\,\,\,\,\,\,\,b = 1 - {1 \over y}$$
<br><br>$$z = \sum\limits_{n = 0}^\infty  {{c^n}}  = {1 \over {1 - c}}\,\,\,\,\,\,\,\,\,\,c = 1 - {1 \over z}$$
<br><br>$$a,b,c$$ are in $$A.P.$$ OR $$2b = a + c$$
<br><br>$$2\left( {1 - {1 \over y}} \right) = 1 - {1 \over x} + 1 - {1 \over y}$$
<br><br>$${2 \over y} = {1 \over x} + {1 \over z} \Rightarrow x,y,z$$ are in $$H.P.$$ 

### Example 2 (Year: 2006)

**Question:**

If $${{a_1},{a_2},....{a_n}}$$ are in H.P., then the expression $${{a_1}\,{a_2} + \,{a_2}\,{a_3}\, + .... + {a_{n - 1}}\,{a_n}}$$ is equal to 

**Solution:**

$${1 \over {{a_2}}} - {1 \over {{a_1}}} = {1 \over {{a_3}}} - {1 \over {{a_2}}} = .........$$
<br><br>$$\,\,\,\,\,\,\,\,\,\,\,\,\,\,\, = {1 \over {{a_n}}} - {1 \over {{a_{n - 1}}}} = d$$ (say)
<br><br>Then $${a_1}{a_2} = {{{a_1} - a{}_2} \over d},\,{a_2}{a_3} = {{{a_2} - {a_3}} \over d},$$
<br><br>$$\,\,\,\,\,\,\,\,\,\,\,\,\,\,\,......,\,{a_{n - 1}}{a_n} = {{{a_{n - 1}} - {a_n}} \over d}$$
<br><br>$$\therefore$$ $${a_1}a{}_2 + {a_2}{a_3} + ......... + {a_{n - 1}}{a_n}$$
<br><br>$$ = {{{a_1} - {a_2}} \over d} + {{{a_2} - {a_3}} \over d} + ......$$
<br><br>$$\,\,\,\,\,\,\,\,\,\,\,\,\,\,\, + {{{a_{n - 1}} - {a_n}} \over d}$$
<br><br>$$ = {1 \over a}\left[ {{a_1}} \right. - {a_2} + {a_2} - {a_3} + .......$$
<br><br>$$\,\,\,\,\,\,\,\,\,\,\,\,\,\,\,\left. { + {a_{n - 1}} - an} \right] = {{{a_1} - {a_n}} \over d}$$
<br><br>Also, $${1 \over {{a_n}}} = {1 \over {{a_1}}} + \left( {n - 1} \right)d$$
<br><br>$$ \Rightarrow {{{a_1} - {a_n}} \over {{a_1}{a_n}}} = \left( {n - 1} \right)d$$
<br><br>$$...

### Example 3 (Year: 2022)

**Question:**

<p>$$x = \sum\limits_{n = 0}^\infty  {{a^n},y = \sum\limits_{n = 0}^\infty  {{b^n},z = \sum\limits_{n = 0}^\infty  {{c^n}} } } $$, where a, b, c are in A.P. and |a| < 1, |b| < 1, |c| < 1, abc $$\ne$$ 0, then :</p>

**Solution:**

<p>$$x = \sum\limits_{n = 0}^\infty  {{a^n} = {1 \over {1 - a}};\,y = \sum\limits_{n = 0}^\infty  {{b^n} = {1 \over {1 - b}};\,z = \sum\limits_{n = 0}^\infty  {{c^n} = {1 \over {1 - c}}} } } $$</p>
<p>Now,</p>
<p>a, b, c $$\to$$ AP</p>
<p>1 $$-$$ a, 1 $$-$$ b, 1 $$-$$ c $$\to$$ AP</p>
<p>$${1 \over {1 - a}},\,{1 \over {1 - b}},\,{1 \over {1 - c}} \to HP$$</p>
<p>x, y, z $$\to$$ HP</p>
<p>$$\therefore$$ $${1 \over x},{1 \over y},{1 \over z} \to AP$$</p>

### Example 4 (Year: 2025)

**Question:**

For positive integers $n$, if $4 a_n=\left(n^2+5 n+6\right)$ and $S_n=\sum\limits_{k=1}^n\left(\frac{1}{a_k}\right)$, then the value of $507 S_{2025}$ is :

**Solution:**

<p>$$\begin{aligned}
\mathrm{a}_{\mathrm{n}} & =\frac{\mathrm{n}^2+5 \mathrm{n}+6}{4} \\
\mathrm{~S}_{\mathrm{n}} & =\mathrm{S}_{\mathrm{n}}=\sum_{\mathrm{k}=1}^{\mathrm{n}} \frac{1}{\mathrm{a}_{\mathrm{k}}}=\sum_1^{\mathrm{n}} \frac{4}{\mathrm{k}^2+5 \mathrm{k}+6} \\
& =4 \sum_{\mathrm{k}=1}^{\mathrm{n}} \frac{1}{(\mathrm{k}+2)(\mathrm{k}+3)} \\
& =4 \sum_{\mathrm{k}=1}^{\mathrm{n}} \frac{1}{\mathrm{k}+2}-\frac{1}{\mathrm{k}+3} \\
& =4\left(\frac{1}{3}-\frac{1}{4}\right)+4\left(\frac{1}{4}-\frac{1}{5}\right)+\ldots \ldots . .
\end{aligned}$$</p>
<p>$$\begin{array}{l}
4\left(\frac{1}{\mathrm{n}+2}-\frac{1}{\mathrm{n}+3}\right) \\
=4\left(\frac{1}{3}-\frac{1}{\mathrm{n}+3}\right) \\
=\frac{4 \mathrm{n}}{3(\mathrm{n}+3)} \\
{ }^{507} \mathrm{~S}_{2025}=\frac{(507)(4)(2025)}{3(2028)} \\
=675
\end{array}$$</p>
