---
chapter: sequences-and-series
topic: arithmetico-geometric-progression
jee_frequency: 4
years_appeared: [2022, 2023, 2024, 2025]
question_count: 7
difficulty: medium
question_types: ['integer', 'mcq']
exams: ['mains']
---

# Sequences And Series: Arithmetico Geometric Progression

**JEE Frequency**: Appeared in **4 years** (2022 - 2025)

**Question Count**: 7 questions

## Question Types

- **INTEGER**: 6 questions
- **MCQ**: 1 questions

## Difficulty Distribution

- **Medium**: 5 questions
- **Easy**: 1 questions
- **Hard**: 1 questions

## Worked Examples

### Example 1 (Year: 2022)

**Question:**

<p>Let for $$f(x) = {a_0}{x^2} + {a_1}x + {a_2},\,f'(0) = 1$$ and $$f'(1) = 0$$. If a<sub>0</sub>, a<sub>1</sub>, a<sub>2</sub> are in an arithmatico-geometric progression, whose corresponding A.P. has common difference 1 and corresponding G.P. has common ratio 2, then f(4) is equal to _____________.</p>

**Solution:**

<p>Given,</p>
<p>$$f(x) = {a_0}{x^2} + {a_1}x + {a_2}$$</p>
<p>$$f'(0) = 1$$</p>
<p>$$f'(1) = 0$$</p>
<p>a<sub>0</sub>, a<sub>1</sub>, a<sub>2</sub> are in A. G. P</p>
<p>Common difference of $$AP = 1$$</p>
<p>Common ratio of $$GP = 2$$</p>
<p>A.P terms = a, a + 1, a + 2</p>
<p>G.P terms = y, ry, r<sup>2</sup>y</p>
<p>$$\therefore$$ AGP terms = ay, (a+1)ry, (a+2)r<sup>2</sup>y</p>
<p>$$\therefore$$ $${a_0} = ay$$</p>
<p>$${a_1} = (a + 1)ry = (a + 1)2y$$</p>
<p>$${a_2} = (a + 2){r^2}y = (a + 2)4y$$</p>
<p>Now, $$f'(x) = 2x{a_0} + {a_1}$$</p>
<p>$$\therefore$$ $$f'(0) = {a_1} = 1$$</p>
<p>and $$f'(1) = 2{a_0} + {a_1} = 0$$</p>
<p>$$ \Rightarrow 2{a_0} + 1 = 0$$</p>
<p>$$ \Rightarrow {a_0} =  - {1 \over 2}$$</p>
<p>$$\therefore$$ $$ay =  - {1 \over 2}$$</p>
<p>and $$(a + 1)2y = 1$$</p>
<p>$$ \Rightarrow 2ay + 2y = 1$$</p>
<p>$$ \Rightarrow 2 \times \left( { - {1 \over 2}} \right) + 2y = 1$$</p>
<p>$$ \Rightarrow 2y =  + \,2$$</p>
<p>$$ \Rightarrow y =  + \,1$$</p>
<p>$$\therefore$$ $$a = ...

### Example 2 (Year: 2023)

**Question:**

<p>Suppose $$a_{1}, a_{2}, 2, a_{3}, a_{4}$$ be in an arithmetico-geometric progression. If the common ratio of the corresponding geometric progression is 2 and the sum of all 5 terms of the arithmetico-geometric progression is $$\frac{49}{2}$$, then $$a_{4}$$ is equal to __________.</p>

**Solution:**

Since, common ratio of A.G.P. is 2 therefore A.G.P. can be taken as
<br/><br/>$$
\begin{aligned}
& \frac{(a-2 d)}{4}, \frac{(c-d)}{2}, a, 2(a+d), 4(a+2 d) \\\\
& \text { or } a_1, a_2, 2, a_3, a_4 \text { (Given) } \\\\
& \Rightarrow a=2
\end{aligned}
$$
<br/><br/>also sum of thes A.G.P. is $\frac{49}{2}$
<br/><br/>$$
\begin{aligned}
& \Rightarrow \frac{2-2 d}{4}+\frac{2-d}{2}+2+2(2+d)+4(2+2 d)=\frac{49}{2} \\\\
& \Rightarrow \frac{1}{4}[2-2 d+4-2 d+8+16+8 d+32+32 d]=\frac{49}{2} \\\\
& \Rightarrow 36 d+62=98
\end{aligned}
$$
<br/><br/>$$
\Rightarrow 36 d=36 \Rightarrow d=1
$$
<br/><br/>Hence, $a_4=4(a+2 d)=4(2+2 \times 1)=16$

### Example 3 (Year: 2023)

**Question:**

<p>Let $$0 < z < y < x$$ be three real numbers such that $$\frac{1}{x}, \frac{1}{y}, \frac{1}{z}$$ are in an arithmetic progression and $$x, \sqrt{2} y, z$$ are in a geometric progression. If $$x y+y z+z x=\frac{3}{\sqrt{2}} x y z$$ , then $$3(x+y+z)^{2}$$ is equal to ____________.</p>

**Solution:**

$\because \frac{1}{x}, \frac{1}{y}, \frac{1}{z}$ are in A.P.
<br/><br/>$$
\Rightarrow \frac{1}{x}+\frac{1}{z}=\frac{2}{y}
$$ ........... (i)
<br/><br/>and $x, \sqrt{2} y, z$ are in G.P.
<br/><br/>$$
\Rightarrow 2 y^2=x z
$$ .......... (ii)
<br/><br/>from (i), $\frac{2}{y}=\frac{x+z}{x z}=\frac{x+z}{2 y^2}$
<br/><br/>$$
\Rightarrow 4 y=x+z
$$
<br/><br/>$$
\begin{aligned}
& \text { Also, } x y+y z+z x=\frac{3}{\sqrt{2}} x y z \\\\
& y(4 y)+x z=\frac{3}{\sqrt{2}}\left(2 y^2\right) y \\\\
& \Rightarrow 4 y^2+2 y^2=3 \sqrt{2} y^3 \\\\
& \Rightarrow 6 y^2=3 \sqrt{2} y^3 \Rightarrow y=\sqrt{2} \\\\
& \therefore 3(x+y+z)^2=3(5 y)^2=3(5 \sqrt{2})^2 \\\\
& =150
\end{aligned}
$$

### Example 4 (Year: 2024)

**Question:**

If $8=3+\frac{1}{4}(3+p)+\frac{1}{4^2}(3+2 p)+\frac{1}{4^3}(3+3 p)+\cdots \cdots \infty$, then the value of $p$ is ____________.

**Solution:**

<p>$$8=\frac{3}{1-\frac{1}{4}}+\frac{p \cdot \frac{1}{4}}{\left(1-\frac{1}{4}\right)^2}$$</p>
<p>$$\text { (sum of infinite terms of A.G.P }=\frac{a}{1-r}+\frac{d r}{(1-r)^2} \text { ) }$$</p>
<p>$$\Rightarrow \frac{4 p}{9}=4 \Rightarrow p=9$$</p>

### Example 5 (Year: 2024)

**Question:**

<p>If $$1+\frac{\sqrt{3}-\sqrt{2}}{2 \sqrt{3}}+\frac{5-2 \sqrt{6}}{18}+\frac{9 \sqrt{3}-11 \sqrt{2}}{36 \sqrt{3}}+\frac{49-20 \sqrt{6}}{180}+\ldots$$ upto $$\infty=2+\left(\sqrt{\frac{b}{a}}+1\right) \log _e\left(\frac{a}{b}\right)$$, where a and b are integers with $$\operatorname{gcd}(a, b)=1$$, then $$\mathrm{11 a+18 b}$$ is equal to __________.</p>

**Solution:**

<p>$$\begin{aligned}
& S=1+\frac{\sqrt{3}-\sqrt{2}}{2 \sqrt{3}}+\frac{5-2 \sqrt{6}}{18}+\frac{9 \sqrt{3}-11 \sqrt{2}}{36 \sqrt{3}}+\ldots \infty \\\\
& =1+\frac{(1-\sqrt{2} / \sqrt{3})}{2}+\frac{(1-\sqrt{2} / \sqrt{3})^2}{6}+\frac{(1-\sqrt{2} / \sqrt{3})^3}{12}+\ldots \infty
\end{aligned}$$</p>
<p>$$\text { let } 1-\frac{\sqrt{2}}{\sqrt{3}}=a$$</p>
<p>$$\begin{aligned}
& S=1+\frac{a}{2}+\frac{a^2}{6}+\frac{a^3}{12}+\ldots \\\\
& =1+\left(1-\frac{1}{2}\right) a+\left(\frac{1}{2}-\frac{1}{3}\right) a^2+\left(\frac{1}{3}-\frac{1}{4}\right) a^3+\ldots \\\\
& =1+\left(a+\frac{a^2}{2}+\frac{a^3}{3} \ldots \infty\right)+\frac{1}{a}\left(\frac{-a^2}{2}-\frac{a^3}{3}-\frac{a^4}{4} \ldots \infty\right) \\\\
& =-\ln (1-a)+\frac{1}{a}\left(-a-\frac{a^2}{2}-\frac{a^3}{3} \ldots \infty\right)+2 \\\\
& =-\ln (1-a)+\frac{1}{a} \ln (1-a)+2 \\\\
& =2+\left(\frac{1}{a}-1\right) \ln (1-a) \\\\
& =2+\left(\frac{\sqrt{3}}{\sqrt{3}-\sqrt{2}}-1\right) \ln \left(1-1+\sqrt{\frac{2}{3}}\right) \\\\
& =2+\frac{\s...
