---
chapter: trigonometric-ratio-and-identites
topic: trigonometric-ratio-of-standard-angles
jee_frequency: 4
years_appeared: [2021, 2022, 2023, 2024]
question_count: 7
difficulty: medium
question_types: ['mcq', 'integer']
exams: ['mains']
---

# Trigonometric Ratio And Identites: Trigonometric Ratio Of Standard Angles

**JEE Frequency**: Appeared in **4 years** (2021 - 2024)

**Question Count**: 7 questions

## Question Types

- **MCQ**: 6 questions
- **INTEGER**: 1 questions

## Difficulty Distribution

- **Medium**: 7 questions

## Worked Examples

### Example 1 (Year: 2021)

**Question:**

The value of $$\cot {\pi  \over {24}}$$ is :

**Solution:**

$$\cot \theta  = {{1 + \cos 2\theta } \over {\sin 2\theta }} = {{1 + \left( {{{\sqrt 3  + 1} \over {2\sqrt 2 }}} \right)} \over {\left( {{{\sqrt 3  - 1} \over {2\sqrt 2 }}} \right)}}$$<br><br>$$\theta  = {\pi  \over {24}}$$<br><br>$$ \Rightarrow \cot \left( {{\pi  \over {24}}} \right) = {{1 + \left( {{{\sqrt 3  + 1} \over {2\sqrt 2 }}} \right)} \over {\left( {{{\sqrt 3  - 1} \over {2\sqrt 2 }}} \right)}}$$<br><br>$$ = {{\left( {2\sqrt 2  + \sqrt 3  + 1} \right)} \over {\left( {\sqrt 3  - 1} \right)}} \times {{\left( {\sqrt 3  + 1} \right)} \over {\left( {\sqrt 3  + 1} \right)}}$$<br><br>$$ = {{2\sqrt 6  + 2\sqrt 2  + 3 + \sqrt 3  + \sqrt 3  + 1} \over 2}$$<br><br>$$ = \sqrt 6  + \sqrt 2  + \sqrt 3  + 2$$

### Example 2 (Year: 2022)

**Question:**

<p>$$\alpha  = \sin 36^\circ $$ is a root of which of the following equation?</p>

**Solution:**

<p>Given that $\alpha = \sin 36^\circ$, we need to determine which equation it is a root of.</p>

<p>We start with the known relationship for $\cos 72^\circ$:</p>

<p>$ \cos 72^\circ = \frac{\sqrt{5}-1}{4} $</p>

<p>Using the double-angle formula for cosine:</p>

<p>$ \cos 72^\circ = 1 - 2 \sin^2 36^\circ $</p>

<p>Substitute $\alpha$ for $\sin 36^\circ$:</p>

<p>$ 1 - 2\alpha^2 = \frac{\sqrt{5}-1}{4} $</p>

<p>Multiply both sides by 4:</p>

<p>$ 4 - 8\alpha^2 = \sqrt{5} - 1 $</p>

<p>Add 1 to both sides:</p>

<p>$ 5 - 8\alpha^2 = \sqrt{5} $</p>

<p>Square both sides to eliminate the radical:</p>

<p>$ (5 - 8\alpha^2)^2 = 5 $</p>

<p>Expand the left side:</p>

<p>$ 25 + 64\alpha^4 - 80\alpha^2 = 5 $</p>

<p>Simplify by subtracting 5 from both sides:</p>

<p>$ 64\alpha^4 - 80\alpha^2 + 20 = 0 $</p>

<p>Divide the entire equation by 4:</p>

<p>$ 16\alpha^4 - 20\alpha^2 + 5 = 0 $</p>

<p>Thus, the equation $16\alpha^4 - 20\alpha^2 + 5 = 0$ is the one for which $\alpha = \sin 36^\circ$ is ...

### Example 3 (Year: 2022)

**Question:**

<p>The value of 2sin (12$$^\circ$$) $$-$$ sin (72$$^\circ$$) is :</p>

**Solution:**

<p>$$2\sin 12^\circ  - \sin 72^\circ $$</p>
<p>$$ = \sin 12^\circ  + ( - 2\cos 42^\circ \,.\,\sin 30^\circ )$$</p>
<p>$$ = \sin 12^\circ  - \cos 42^\circ $$</p>
<p>$$ = \sin 12^\circ  - \sin 48^\circ $$</p>
<p>$$ = 2\sin 18^\circ \,.\,\cos 30^\circ $$</p>
<p>$$ =  - 2\left( {{{\sqrt 5  - 1} \over 4}} \right)\,.\,{{\sqrt 3 } \over 2}$$</p>
<p>$$ = {{\sqrt 3 \left( {1 - \sqrt 5 } \right)} \over 4}$$</p>

### Example 4 (Year: 2023)

**Question:**

<p>If $$\tan 15^\circ  + {1 \over {\tan 75^\circ }} + {1 \over {\tan 105^\circ }} + \tan 195^\circ  = 2a$$, then the value of $$\left( {a + {1 \over a}} \right)$$ is :</p>

**Solution:**

<p>$$\tan 15^\circ  + \tan 15^\circ  - \tan 15^\circ  + \tan 15^\circ $$</p>
<p>$$ = 2\tan 15^\circ $$</p>
<p>$$ = 2\left( {2 - \sqrt 3 } \right) = 2a \Rightarrow a = 2 - \sqrt 3 $$</p>
<p>$$\therefore$$ $${1 \over a} + a \Rightarrow \left( {2 + \sqrt 3 } \right) + \left( {2 - \sqrt 3 } \right) = 4$$</p>

### Example 5 (Year: 2023)

**Question:**

<p>The value of $$36\left(4 \cos ^{2} 9^{\circ}-1\right)\left(4 \cos ^{2} 27^{\circ}-1\right)\left(4 \cos ^{2} 81^{\circ}-1\right)\left(4 \cos ^{2} 243^{\circ}-1\right)$$ is :</p>

**Solution:**

$$
\begin{aligned}
& 4 \cos ^2 \theta-1=4\left(1-\sin ^2 \theta\right)-1 \\\\
& =3-4 \sin ^2 \theta \\\\
& =\frac{3 \sin \theta-4 \sin ^3 \theta}{\sin \theta} \\\\
& =\frac{\sin 3 \theta}{\sin \theta}
\end{aligned}
$$
<br/><br/>$$36\left(4 \cos ^{2} 9^{\circ}-1\right)\left(4 \cos ^{2} 27^{\circ}-1\right)\left(4 \cos ^{2} 81^{\circ}-1\right)\left(4 \cos ^{2} 243^{\circ}-1\right)$$
<br/><br/>$$
\begin{aligned}
& =36\left[\frac{\sin 27^{\circ}}{\sin 9^{\circ}} \times \frac{\sin 81^{\circ}}{\sin 27^{\circ}} \times \frac{\sin 243^{\circ}}{\sin 81^{\circ}} \times \frac{\sin 729^{\circ}}{\sin 243^{\circ}}\right] \\\\
& =36\left[\frac{\sin 729^{\circ}}{\sin 9^{\circ}}\right]=36 \times 1=36
\end{aligned}
$$
