---
chapter: trigonometric-ratio-and-identites
topic: summation-series-problems
jee_frequency: 2
years_appeared: [2020, 2021]
question_count: 2
difficulty: medium
question_types: ['mcq']
exams: ['mains']
---

# Trigonometric Ratio And Identites: Summation Series Problems

**JEE Frequency**: Appeared in **2 years** (2020 - 2021)

**Question Count**: 2 questions

## Question Types

- **MCQ**: 2 questions

## Difficulty Distribution

- **Medium**: 2 questions

## Worked Examples

### Example 1 (Year: 2020)

**Question:**

If $$x = \sum\limits_{n = 0}^\infty  {{{\left( { - 1} \right)}^n}{{\tan }^{2n}}\theta } $$ and  $$y = \sum\limits_{n = 0}^\infty  {{{\cos }^{2n}}\theta } $$<br><br> for
0 &lt; $$\theta $$ &lt; $${\pi  \over 4}$$, then :

**Solution:**

$$x = \sum\limits_{n = 0}^\infty  {{{\left( { - 1} \right)}^n}{{\tan }^{2n}}\theta } $$
<br><br>= 1 – tan<sup>2</sup>$$\theta $$ + tan<sup>2</sup> 4$$\theta $$ + ...
<br><br>= $${1 \over {1 + {{\tan }^2}\theta }}$$ = cos<sup>2</sup> $$\theta $$ ....(1)
<br><br>$$y = \sum\limits_{n = 0}^\infty  {{{\cos }^{2n}}\theta } $$
<br><br>=  1 + cos<sup>2</sup>
$$\theta $$ + cos<sup>4</sup>
$$\theta $$ + cos<sup>6</sup>
$$\theta $$ + ....
<br><br>= $${1 \over {1 - {{\cos }^2}\theta }}$$ = $${1 \over {{{\sin }^2}\theta }}$$
<br><br>$$ \Rightarrow $$ sin<sup>2</sup> $$\theta $$ = $${1 \over y}$$ ...(2)
<br><br>Adding (1) and (2), we get, 
<br><br>x + $${1 \over y}$$ = sin<sup>2</sup> $$\theta $$ + cos<sup>2</sup> $$\theta $$
<br><br>$$ \Rightarrow $$ x + $${1 \over y}$$ = 1
<br><br>$$ \Rightarrow $$ y(1 – x) = 1

### Example 2 (Year: 2021)

**Question:**

If
$${e^{\left( {{{\cos }^2}x + {{\cos }^4}x + {{\cos }^6}x + ...\infty } \right){{\log }_e}2}}$$
satisfies the equation t<sup>2</sup> - 9t + 8 = 0, then the value of
<br>$${{2\sin x} \over {\sin x + \sqrt 3 \cos x}}\left( {0 &lt; x &lt; {\pi  \over 2}} \right)$$ is :

**Solution:**

$${e^{({{\cos }^2}x + {{\cos }^4}x + ...........\infty )\ln 2}} = {2^{{{\cos }^2}x + {{\cos }^4}x + ...........\infty }}$$
<br><br>= $${2^{{{{{\cos }^2}x} \over {1 - {{\cos }^2}x}}}}$$
<br><br>$$ = {2^{{{\cot }^2}x}}$$<br><br>Given, $${t^2} - 9t + 8 = 0 \Rightarrow t = 1,8$$<br><br>$$ \Rightarrow {2^{{{\cot }^2}x}} = 1,8 \Rightarrow co{t^2}x = 0,3$$<br><br>$$0 &lt; x &lt; {\pi  \over 2} \Rightarrow \cot x = \sqrt 3 $$<br><br>$$ \therefore $$ $$  {{2\sin x} \over {\sin x + \sqrt 3 \cos x}} = {2 \over {1 + \sqrt 3 \cot x}} = {2 \over 4} = {1 \over 2}$$
