---
chapter: trigonometric-ratio-and-identites
topic: fundamental-identities
jee_frequency: 7
years_appeared: [2006, 2013, 2014, 2019, 2021, 2024, 2025]
question_count: 10
difficulty: medium
question_types: ['mcq']
exams: ['mains']
---

# Trigonometric Ratio And Identites: Fundamental Identities

**JEE Frequency**: Appeared in **7 years** (2006 - 2025)

**Question Count**: 10 questions

## Question Types

- **MCQ**: 10 questions

## Difficulty Distribution

- **Medium**: 8 questions
- **Easy**: 2 questions

## Worked Examples

### Example 1 (Year: 2006)

**Question:**

If $$0 &lt; x &lt; \pi $$ and $$\cos x + \sin x = {1 \over 2},$$ then $$\tan x$$ is :

**Solution:**

$$\cos x + \sin x = {1 \over 2}$$ <br><br>
$$ \Rightarrow {\left( {\cos x + {\mathop{\rm sinx}\nolimits} } \right)^2} = {1 \over 4}$$<br><br>
$$ \Rightarrow {\cos ^2}x + {\sin ^2}x + 2\cos x\sin x = {1 \over 4}$$<br>
$$\left[ \because {{{\cos }^2}x + {{\sin }^2}x = 1\, \,and \,\,2\cos x\sin x = \sin 2x} \right]$$
<br><br>$$ \Rightarrow 1 + \sin 2x = {1 \over 4}$$
<br><br>$$ \Rightarrow \sin 2x =  - {3 \over 4},$$ so $$x$$ is obtuse and 
<br><br>$${{2\tan x} \over {1 + {{\tan }^2}x}} =  - {3 \over 4}$$
<br><br>$$ \Rightarrow 3{\tan ^2}x + 8\tan x + 3 = 0$$
<br><br>$$\therefore$$ $$\tan x = {{ - 8 \pm \sqrt {64 - 36} } \over 6}$$
<br><br>$$ = {{ - 4 \pm \sqrt 7 } \over 3}$$
<br><br>as $$\tan x &lt; 0\,$$ 
<br><br>$$\therefore$$ $$\tan x = {{ - 4 - \sqrt 7 } \over 3}$$ 

### Example 2 (Year: 2013)

**Question:**

The expression $${{\tan {\rm A}} \over {1 - \cot {\rm A}}} + {{\cot {\rm A}} \over {1 - \tan {\rm A}}}$$  can be written as: 

**Solution:**

Given expression can be written as 
<br><br>$${{\sin A} \over {\cos A}} \times {{sin\,A} \over {\sin A - \cos A}} + {{\cos A} \over {\sin A}} \times {{\cos A} \over {\cos A - sin\,A}}$$
<br><br>(As $$\tan A = {{\sin A} \over {\cos A}}$$ and $$\cot A = {{\cos A} \over {\sin A}}$$ )
<br><br>$$ = {1 \over {\sin A - \cos A}}\left\{ {{{{{\sin }^3}A - {{\cos }^3}A} \over {\cos A\sin A}}} \right\}$$
<br><br>$$ = {{{{\sin }^2}A + \sin A\cos A + {{\cos }^2}\,A} \over {\sin A\cos A}}$$
<br><br>$$ = 1 + \sec\, A{\mathop{\rm cosec}\nolimits} \,A$$ 

### Example 3 (Year: 2014)

**Question:**

Let $$f_k\left( x \right) = {1 \over k}\left( {{{\sin }^k}x + {{\cos }^k}x} \right)$$ where $$x \in R$$ and $$k \ge \,1.$$
<br>Then $${f_4}\left( x \right) - {f_6}\left( x \right)\,\,$$ equals :

**Solution:**

Let $${f_k}\left( x \right) = {1 \over k}\left( {{{\sin }^k}x + {{\cos }^k}.x} \right)$$
<br><br>Consider 
<br><br>$${f_4}\left( x \right) - {f_6}\left( x \right)  $$
<br><br>$$=$$ $${1 \over 4}\left( {{{\sin }^4}x + {{\cos }^4}x} \right) - {1 \over 6}\left( {{{\sin }^6}x + {{\cos }^6}x} \right)$$
<br><br>$$ = {1 \over 4}\left[ {1 - 2{{\sin }^2}x{{\cos }^2}x} \right] - {1 \over 6}\left[ {1 - 3{{\sin }^2}x{{\cos }^2}x} \right]$$
<br><br>$$ = {1 \over 4} - {1 \over 6} = {1 \over {12}}$$

### Example 4 (Year: 2019)

**Question:**

For any  $$\theta  \in \left( {{\pi  \over 4},{\pi  \over 2}} \right)$$, the expression
<br><br> $$3{(\cos \theta  - \sin \theta )^4}$$$$ + 6{(\sin \theta  + \cos \theta )^2} + 4{\sin ^6}\theta $$ 
<br><br>equals :

**Solution:**

Given, 
<br><br>3(sin$$\theta $$ $$-$$ cos$$\theta $$)<sup>4</sup> + 6(sin$$\theta $$ + cos$$\theta $$)<sup>2</sup> + 4sin<sup>6</sup>$$\theta $$
<br><br>=  3[(sin$$\theta $$ $$-$$ cos$$\theta $$)<sup>2</sup>]<sup>2</sup> + 6 (sin<sup>2</sup>$$\theta $$ + cos<sup>2</sup>$$\theta $$ + 2sin$$\theta $$cos$$\theta $$) + 4sin<sup>6</sup>$$\theta $$
<br><br>=  3[sin<sup>2</sup>$$\theta $$ + cos<sup>2</sup>$$\theta $$ $$-$$2sin$$\theta $$cos$$\theta $$]<sup>2</sup> + 6(1 + sin2$$\theta $$) + 4sin<sup>6</sup>$$\theta $$
<br><br>=  3(1 $$-$$ sin2$$\theta $$)<sup>2</sup> + 6(1 + sin2$$\theta $$) + 4sin<sup>6</sup>$$\theta $$
<br><br>=  3 (1 $$-$$ 2 sin2$$\theta $$ + sin<sup>2</sup>2$$\theta $$) + 6 + 6sin2$$\theta $$ + 4sin<sup>6</sup>$$\theta $$
<br><br>=  3 $$-$$ 6sin2$$\theta $$ + 3sin<sup>2</sup>2$$\theta $$ + 6 + 6sin2$$\theta $$ + 4sin<sup>6</sup>$$\theta $$
<br><br>=  9 + 3sin<sup>2</sup>2$$\theta $$ + 4 sin<sup>6</sup>$$\theta $$
<br><br>=  9 + 3(2sin$$\theta $$cos$$\theta $$)<sup>2</sup...

### Example 5 (Year: 2021)

**Question:**

If for x $$\in$$ $$\left( {0,{\pi  \over 2}} \right)$$, log<sub>10</sub>sinx + log<sub>10</sub>cosx = $$-$$1 and log<sub>10</sub>(sinx + cosx) = $${1 \over 2}$$(log<sub>10</sub> n $$-$$ 1), n &gt; 0, then the value of n is equal to :

**Solution:**

$$
\begin{aligned}
& \log _{10} \sin x+\log _{10} \cos x=-1, x \in(0, \pi / 2) \\\\
& \log _{10}(\sin x \cos x)=-1 \\\\
& \Rightarrow  \sin x \cos x=10^{-1}= {1 \over {10}} \\\\
& \log _{10}(\sin x+\cos x)={1 \over {2}}\left(\log _{10} n-1\right), n>0 \\\\
& 2 \log _{10}(\sin x+\cos x)=\left(\log _{10} n-\log _{10} 10\right) \\\\
& \Rightarrow \log _{10}(\sin x+\cos x)^2=\log _{10}({n \over {10}}) \\\\
& \Rightarrow (\sin x+\cos x)^2={n \over {10}} \\\\
& \Rightarrow \sin ^2 x+\cos ^2 x+2 \sin x \cos x=\frac{n}{10} \\\\
& \Rightarrow 1+2({1 \over {10}})={n \over {10}} \Rightarrow {12 \over {10}}={n \over {10}} \\\\
& \therefore n=12
\end{aligned}
$$
